ported GC

Test/civl/large-samples/GC.bpl
@@ -5,50 +5,39 @@
 // RUN: %parallel-boogie "%s" > "%t"
 // RUN: %diff "%s.expect" "%t"
 
-type {:linear "tid"} X = int;
-function {:inline} Subset(X: [X]bool, Y: [X]bool) : (bool)
-{
-    MapOr(MapNot(X), Y) == MapConst(true)
-}
-
-// Tid(i, left, right) represents a linear thread id for thread number i, where i > 0.
+// Tid(i, ps) represents a linear thread id for thread number i, where i > 0 and ps = {Left(i), Right(i)}.
 // Thread ids can be split into left and right fractions:
-//   - For a whole thread id, both the left and right fields are true.
-//   - For a fraction, either the left or right field is true.
-// In other words, Tid(i, true, true) can be be split into Tid(i, true, false), Tid(i, false, true).
-datatype Tid { Tid(i:int, left:bool, right:bool) }
-
-function {:inline} {:linear "tid"} TidCollector(x: Tid) : [X]bool
-{
-    MapConst(false)[-x->i := x->left][x->i := x->right]
-}
+//   - For a whole thread id, both Left(i) and Right(i) are in ps.
+//   - For a fraction, either Left(i) or Right(i) is in ps.
+// In other words, Tid(i, { Left(i), Right(i) }) can be be split into Tid(i, { Left(i) }), Tid(i, { Right(i) }).
+datatype Piece { Left(i:int), Right(i:int) }
+datatype Tid { Tid(i:int, {:linear} ps: Set Piece) }
 
 const numMutators: int;
 axiom 0 < numMutators;
 const GcTid: Tid;
-axiom numMutators < GcTid->i && GcTid->left && GcTid->right;
+axiom numMutators < GcTid->i;
+axiom Set_Contains(GcTid->ps, Left(GcTid->i)) && Set_Contains(GcTid->ps, Right(GcTid->i));
 
 function mutatorId(i: int) : bool { 1 <= i && i <= numMutators }
 function mutatorTid(tid: Tid) : bool { mutatorId(tid->i) }
-function mutatorTidLeft(tid: Tid) : bool { mutatorTid(tid) && tid->left }
-function mutatorTidRight(tid: Tid) : bool { mutatorTid(tid) && tid->right }
-function mutatorTidWhole(tid: Tid) : bool { mutatorTid(tid) && tid->left && tid->right }
-function gcAndMutatorTids(tid: Tid, mutatorTids: [int]bool) : bool
+function mutatorTidLeft(tid: Tid) : bool { mutatorTid(tid) && Set_Contains(tid->ps, Left(tid->i)) }
+function mutatorTidRight(tid: Tid) : bool { mutatorTid(tid) && Set_Contains(tid->ps, Right(tid->i)) }
+function mutatorTidWhole(tid: Tid) : bool { mutatorTid(tid) && Set_Contains(tid->ps, Left(tid->i)) && Set_Contains(tid->ps, Right(tid->i)) }
+function gcAndMutatorTids(tid: Tid, mutatorTids: Set Piece) : bool
 {
-    tid == GcTid && (forall i:int :: mutatorId(i) ==> mutatorTids[i] && mutatorTids[-i])
+    tid == GcTid && (forall i:int :: mutatorId(i) ==> Set_Contains(mutatorTids, Left(i)) && Set_Contains(mutatorTids, Right(i)))
 }
 
-function Size([int]bool) returns (int);
-const Mutators: [int]bool;
-axiom Size(Mutators) == numMutators;
-axiom Size(MapConst(false)) == 0;
-axiom (forall X, Y: [int]bool :: Subset(X, Y) ==> Size(X) < Size(Y) || X == Y);
-axiom (forall X: [int]bool, x: int ::{Size(X[x := false]), Size(X[x := true])} Size(X[x := false]) + 1 == Size(X[x := true]));
-axiom (forall x: int :: Mutators[x] <==> 1 <= x && x <= numMutators);
-function {:inline} RootScanBarrierInv(Set:[int]bool, rootScanBarrier: int) : bool
+const Mutators: Set Piece;
+axiom Set_Size(Mutators) == numMutators;
+axiom Mutators->val == (lambda x: Piece :: x is Right && 1 <= x->i && x->i <= numMutators);
+axiom (forall X, Y: Set Piece :: Set_IsSubset(X, Y) ==> Set_Size(X) < Set_Size(Y) || X == Y);
+
+function {:inline} RootScanBarrierInv(mutatorsInRootScanBarrier: Set Piece, rootScanBarrier: int) : bool
 {
-    Size(Set) + rootScanBarrier == numMutators &&
-    Subset(Set, Mutators)
+    Set_Size(mutatorsInRootScanBarrier) + rootScanBarrier == numMutators &&
+    Set_IsSubset(mutatorsInRootScanBarrier, Mutators)
 }
 
 type idx = int;
@@ -82,13 +71,13 @@ var {:layer 0,100} mem: [int][fld]int;
 var {:layer 95,100} toAbs: [int]obj;
 var {:layer 0,100} Color: [int]int;
 var {:layer 0,100} collectorPhase: int;
-var {:layer 0,100} mutatorPhase: [X]int;
+var {:layer 0,100} mutatorPhase: [int]int;
 var {:layer 0,100} sweepPtr: int;
 
 // Next layer
 var {:layer 0,99} rootScanOn: bool;
 var {:layer 0,99} rootScanBarrier: int;
-var {:linear "tid"} {:layer 95,99} mutatorsInRootScanBarrier: [int]bool;
+var {:linear} {:layer 95,99} mutatorsInRootScanBarrier: Set Piece;
 var {:layer 0,98} MarkStack: [int]int;
 var {:layer 0,98} MarkStackPtr: int;
 
@@ -97,7 +86,7 @@ var {:layer 0,98} MarkStackPtr: int;
 var {:layer 95,96} absLock: int; // 0 if unheld; thread number of holder if held
 var {:layer 0,95} lock: bool; // false if unheld; true if held
 
-function tidHasLock(tid:Tid, lock:int):bool { (tid == GcTid || mutatorTid(tid)) && lock == tid->i && tid->left }
+function tidHasLock(tid:Tid, lock:int):bool { (tid == GcTid || mutatorTid(tid)) && lock == tid->i && Set_Contains(tid->ps, Left(tid->i)) }
 
 const memLo: int;
 const memHi: int;
@@ -120,7 +109,7 @@ axiom memAddrAbs(Null());
 axiom (forall i:int :: memAddrAbs(Obj(i)));
 axiom (forall i:int :: !memAddrAbs(Int(i)));
 
-function owner(x: idx): X;
+function owner(x: idx): int;
 function tidOwns(tid:Tid, x:idx):bool { owner(x) == tid->i }
 
 function {:inline} Iso(root:[idx]int, rootAbs:[idx]obj, mem:[int][fld]int, memAbs:[obj][fld]obj, Color:[int]int, toAbs:[int]obj, allocSet:[obj]bool) returns (bool)
@@ -179,14 +168,14 @@ function {:inline} SweepInvInit(root:[idx]int, rootAbs:[idx]obj, mem:[int][fld]i
 // Layer 100
 //////////////////////////////////////////////////////////////////////////////
 
-yield invariant {:layer 100} Yield_WriteField({:linear "tid"} tid:Tid, x: idx, y: idx);
+yield invariant {:layer 100} Yield_WriteField({:linear} tid:Tid, x: idx, y: idx);
 invariant mutatorTidWhole(tid) && tidOwns(tid, x) && tidOwns(tid, y);
 invariant memAddr(root[y]) && MarkPhase(mutatorPhase[tid->i]) ==> Gray(Color[root[y]]) || Black(Color[root[y]]);
 
 yield invariant {:layer 100} Yield_Iso();
 invariant Iso(root, rootAbs, mem, memAbs, Color, toAbs, allocSet);
 
-yield invariant {:layer 100} Yield_GarbageCollect_100({:linear "tid"} tid:Tid);
+yield invariant {:layer 100} Yield_GarbageCollect_100({:linear} tid:Tid);
 invariant tid == GcTid;
 invariant (forall x: int :: memAddr(x) ==> (toAbs[x] == nil <==> Unalloc(Color[x])));
 invariant sweepPtr == memHi ==> (forall x: int :: memAddr(x) ==> !Black(Color[x]));
@@ -195,15 +184,15 @@ invariant sweepPtr == memLo ==>
             (forall i: int :: rootAddr(i) && memAddr(root[i]) ==> Black(Color[root[i]])) &&
             (forall x: int, f: fld :: memAddr(x) && Black(Color[x]) && fieldAddr(f) && memAddr(mem[x][f]) ==> Black(Color[mem[x][f]]));
 
-yield invariant {:layer 100} Yield_CollectorPhase_100({:linear "tid"} tid:Tid, tick_collectorPhase: int);
+yield invariant {:layer 100} Yield_CollectorPhase_100({:linear} tid:Tid, tick_collectorPhase: int);
 invariant tid == GcTid;
 invariant tick_collectorPhase == collectorPhase;
 
-yield invariant {:layer 100} Yield_SweepPtr_100({:linear "tid"} tid:Tid, tick_sweepPtr: int);
+yield invariant {:layer 100} Yield_SweepPtr_100({:linear} tid:Tid, tick_sweepPtr: int);
 invariant tid == GcTid;
 invariant tick_sweepPtr == sweepPtr;
 
-yield invariant {:layer 100} Yield_MarkBegin({:linear "tid"} tid:Tid, tick_Color: [int]int);
+yield invariant {:layer 100} Yield_MarkBegin({:linear} tid:Tid, tick_Color: [int]int);
 invariant tid == GcTid;
 invariant MarkPhase(collectorPhase) && PhaseConsistent(collectorPhase, mutatorPhase) && sweepPtr == memHi;
 invariant (forall x: int :: memAddr(x) ==> (toAbs[x] == nil <==> Unalloc(Color[x])));
@@ -211,21 +200,21 @@ invariant (forall x: int :: memAddr(x) ==> !Black(Color[x]));
 invariant (forall x: int :: memAddr(x) && !Unalloc(tick_Color[x]) ==> !Unalloc(Color[x]));
 invariant (forall x: int :: memAddr(x) && !Unalloc(tick_Color[x]) && !White(tick_Color[x]) ==> !White(Color[x]));
 
-yield invariant {:layer 100} Yield_Mark({:linear "tid"} tid:Tid, tick_Color: [int]int);
+yield invariant {:layer 100} Yield_Mark({:linear} tid:Tid, tick_Color: [int]int);
 invariant tid == GcTid;
 invariant MarkPhase(collectorPhase) && PhaseConsistent(collectorPhase, mutatorPhase) && sweepPtr == memLo;
 invariant MarkInv(root, rootAbs, mem, memAbs, Color, toAbs, allocSet);
 invariant (forall x: int :: memAddr(x) && !Unalloc(tick_Color[x]) ==> !Unalloc(Color[x]));
 invariant (forall x: int :: memAddr(x) && !Unalloc(tick_Color[x]) && !White(tick_Color[x]) ==> !White(Color[x]));
 
-yield invariant {:layer 100} Yield_MarkEnd({:linear "tid"} tid:Tid);
+yield invariant {:layer 100} Yield_MarkEnd({:linear} tid:Tid);
 invariant tid == GcTid;
 invariant MarkPhase(collectorPhase) && PhaseConsistent(collectorPhase, mutatorPhase) && sweepPtr == memLo;
 invariant MarkInv(root, rootAbs, mem, memAbs, Color, toAbs, allocSet);
 invariant (forall x: int :: memAddr(x) ==> !Gray(Color[x]));
 invariant (forall i: int :: rootAddr(i) && memAddr(root[i]) ==> Black(Color[root[i]]));
 
-yield invariant {:layer 100} Yield_MarkInnerLoopFieldIter({:linear "tid"} tid:Tid, fldIter: int, nodeProcessed: int);
+yield invariant {:layer 100} Yield_MarkInnerLoopFieldIter({:linear} tid:Tid, fldIter: int, nodeProcessed: int);
 invariant tid == GcTid;
 invariant 0 <= fldIter && fldIter <= numFields;
 invariant MarkPhase(collectorPhase) && PhaseConsistent(collectorPhase, mutatorPhase) && sweepPtr == memLo;
@@ -233,7 +222,7 @@ invariant MarkInv(root, rootAbs, mem, memAbs, Color, toAbs, allocSet);
 invariant !Unalloc(Color[nodeProcessed]);
 invariant (forall x: int :: 0 <= x && x < fldIter && memAddr(mem[nodeProcessed][x]) ==> !Unalloc(Color[mem[nodeProcessed][x]]) && !White(Color[mem[nodeProcessed][x]]));
 
-yield invariant {:layer 100} Yield_SweepBegin({:linear "tid"} tid:Tid, isInit: bool, tick_Color: [int]int);
+yield invariant {:layer 100} Yield_SweepBegin({:linear} tid:Tid, isInit: bool, tick_Color: [int]int);
 invariant tid == GcTid;
 invariant SweepPhase(collectorPhase) && PhaseConsistent(collectorPhase, mutatorPhase);
 invariant sweepPtr == memLo;
@@ -242,33 +231,33 @@ invariant isInit ==> SweepInvInit(root, rootAbs, mem, memAbs, Color, toAbs, allo
 invariant (forall i: int :: rootAddr(i) && memAddr(root[i]) ==> Black(Color[root[i]]));
 invariant (forall x: int :: memAddr(x) && !Unalloc(tick_Color[x]) ==> tick_Color[x] == Color[x]);
 
-yield invariant {:layer 100} Yield_SweepEnd({:linear "tid"} tid:Tid);
+yield invariant {:layer 100} Yield_SweepEnd({:linear} tid:Tid);
 invariant tid == GcTid;
 invariant SweepPhase(collectorPhase) && PhaseConsistent(collectorPhase, mutatorPhase);
 invariant sweepPtr == memHi;
 invariant SweepInv(root, rootAbs, mem, memAbs, Color, toAbs, allocSet);
 invariant (forall x: int :: memAddr(x) ==> !Black(Color[x]));
 
-yield invariant {:layer 100} Yield_Initialize_100({:linear "tid"} tid:Tid, {:linear "tid"} mutatorTids:[int]bool);
+yield invariant {:layer 100} Yield_Initialize_100({:linear} tid:Tid, {:linear} mutatorTids:Set Piece);
 invariant gcAndMutatorTids(tid, mutatorTids);
 invariant (forall x: idx :: rootAddr(x) ==> rootAbs[x] == Int(0));
 
 yield procedure {:layer 100}
-Initialize({:layer 95, 100} {:linear_in "tid"} tid:Tid, {:layer 95, 100} {:linear "tid"} mutatorTids:[int]bool)
+Initialize({:layer 95, 100} {:linear_in} tid:Tid, {:layer 95, 100} {:linear} mutatorTids:Set Piece)
 requires {:layer 97,98,99} gcAndMutatorTids(tid, mutatorTids);
 requires call Yield_Initialize_100(tid, mutatorTids);
-requires call Yield_InitVars99(mutatorTids, MapConst(false) : [int]bool, old(rootScanBarrier));
+requires call Yield_InitVars99(mutatorTids, Set_Empty(), old(rootScanBarrier));
 requires call Yield_Lock();
 ensures call Yield_Iso();
 ensures call Yield_RootScanBarrierInv();
-ensures call Yield_InitVars99(mutatorTids, MapConst(false) : [int]bool, numMutators);
+ensures call Yield_InitVars99(mutatorTids, Set_Empty(), numMutators);
 {
     par InitVars99(tid, mutatorTids) | Yield_Lock();
     par InitVars100(tid, mutatorTids) | Yield_Lock();
     async call GarbageCollect(tid);
 }
 
-atomic action {:layer 101} AtomicAlloc({:linear "tid"} tid:Tid, i: int, y:idx)
+atomic action {:layer 101} AtomicAlloc({:linear} tid:Tid, i: int, y:idx)
 modifies allocSet, rootAbs, memAbs;
 {
     var o: obj;
@@ -280,7 +269,7 @@ modifies allocSet, rootAbs, memAbs;
 }
 
 yield procedure {:layer 100}
-Alloc({:layer 95, 100} {:linear "tid"} tid:Tid, i: int, y:idx)
+Alloc({:layer 95, 100} {:linear} tid:Tid, i: int, y:idx)
 refines AtomicAlloc;
 requires {:layer 95,96,99,100} mutatorTidWhole(tid);
 preserves call Yield_Iso();
@@ -300,12 +289,12 @@ requires {:layer 96} tid->i == i;
     assert {:layer 100} Iso(root, rootAbs, mem, memAbs, Color, toAbs, allocSet);
 }
 
-atomic action {:layer 101} AtomicWriteField({:linear "tid"} tid:Tid, i: int, x: idx, f: fld, y: idx) // x.f = y
+atomic action {:layer 101} AtomicWriteField({:linear} tid:Tid, i: int, x: idx, f: fld, y: idx) // x.f = y
 modifies memAbs;
 { assert mutatorTidWhole(tid) && rootAddr(x) && tidOwns(tid, x) && fieldAddr(f) && rootAddr(y) && tidOwns(tid, y) && memAddrAbs(rootAbs[x]); memAbs[rootAbs[x]][f] := rootAbs[y]; }
 
 yield procedure {:layer 100}
-WriteField({:layer 95, 100} {:linear "tid"} tid:Tid, i: int, x: idx, f: fld, y: idx)
+WriteField({:layer 95, 100} {:linear} tid:Tid, i: int, x: idx, f: fld, y: idx)
 refines AtomicWriteField;
 requires {:layer 98, 100} mutatorTidWhole(tid);
 preserves call Yield_Iso();
@@ -317,23 +306,23 @@ requires {:layer 95, 96, 99} tid->i == i;
     par WriteFieldRaw(tid, x, f, y) | Yield_Lock();
 }
 
-atomic action {:layer 101} AtomicReadField({:linear "tid"} tid:Tid, x: idx, f: fld, y: idx) // y = x.f
+atomic action {:layer 101} AtomicReadField({:linear} tid:Tid, x: idx, f: fld, y: idx) // y = x.f
 modifies rootAbs;
 { assert mutatorTidWhole(tid) && rootAddr(x) && tidOwns(tid, x) && fieldAddr(f) && rootAddr(y) && tidOwns(tid, y) && memAddrAbs(rootAbs[x]); rootAbs[y] := memAbs[rootAbs[x]][f]; }
 
 yield procedure {:layer 100}
-ReadField({:layer 95, 100} {:linear "tid"} tid:Tid, x: idx, f: fld, y: idx)
+ReadField({:layer 95, 100} {:linear} tid:Tid, x: idx, f: fld, y: idx)
 refines AtomicReadField;
 preserves call Yield_Iso();
 {
     call ReadFieldRaw(tid, x, f, y);
 }
 
-atomic action {:layer 101} AtomicEq({:linear "tid"} tid:Tid, x: idx, y:idx) returns (isEqual:bool)
+atomic action {:layer 101} AtomicEq({:linear} tid:Tid, x: idx, y:idx) returns (isEqual:bool)
 { assert mutatorTidWhole(tid) && rootAddr(x) && tidOwns(tid, x) && rootAddr(y) && tidOwns(tid, y); isEqual := rootAbs[x] == rootAbs[y]; }
 
 yield procedure {:layer 100}
-Eq({:layer 95, 100} {:linear "tid"} tid:Tid, x: idx, y:idx) returns (isEqual:bool)
+Eq({:layer 95, 100} {:linear} tid:Tid, x: idx, y:idx) returns (isEqual:bool)
 refines AtomicEq;
 preserves call Yield_Iso();
 {
@@ -341,7 +330,7 @@ preserves call Yield_Iso();
 }
 
 yield procedure {:layer 100}
-GarbageCollect({:layer 95, 100} {:linear "tid"} tid:Tid)
+GarbageCollect({:layer 95, 100} {:linear} tid:Tid)
 requires {:layer 97,98,99,100} tid == GcTid;
 requires call Yield_Iso();
 requires call Yield_MsWellFormed(tid, 0);
@@ -388,7 +377,7 @@ requires call Yield_Lock();
 }
 
 yield procedure {:layer 100}
-MarkOuterLoop({:layer 95, 100} {:linear "tid"} tid:Tid)
+MarkOuterLoop({:layer 95, 100} {:linear} tid:Tid)
 preserves call Yield_Iso();
 requires call Yield_MarkBegin(tid, old(Color));
 ensures call Yield_MarkEnd(tid);
@@ -418,7 +407,7 @@ preserves call Yield_Lock();
 }
 
 yield procedure {:layer 100}
-MarkInnerLoop({:layer 95, 100} {:linear "tid"} tid:Tid)
+MarkInnerLoop({:layer 95, 100} {:linear} tid:Tid)
 preserves call Yield_Iso();
 preserves call Yield_Mark(tid, old(Color));
 preserves call Yield_MsWellFormed(tid, 0);
@@ -465,7 +454,7 @@ preserves call Yield_Lock();
 }
 
 yield procedure {:layer 100}
-Sweep({:layer 95, 100} {:linear "tid"} tid:Tid)
+Sweep({:layer 95, 100} {:linear} tid:Tid)
 requires {:layer 98,99,100} tid == GcTid;
 preserves call Yield_Iso();
 preserves call Yield_MsWellFormed(tid, 0);
@@ -502,36 +491,36 @@ preserves call Yield_Lock();
 // Layer 99
 //////////////////////////////////////////////////////////////////////////////
 
-yield invariant {:layer 99} Yield_CollectorPhase_99({:linear "tid"} tid:Tid, tick_collectorPhase: int);
+yield invariant {:layer 99} Yield_CollectorPhase_99({:linear} tid:Tid, tick_collectorPhase: int);
 invariant tid == GcTid;
 invariant tick_collectorPhase == collectorPhase;
 
-yield invariant {:layer 99} Yield_SweepPtr_99({:linear "tid"} tid:Tid, tick_sweepPtr: int);
+yield invariant {:layer 99} Yield_SweepPtr_99({:linear} tid:Tid, tick_sweepPtr: int);
 invariant tid == GcTid;
 invariant tick_sweepPtr == sweepPtr;
 
 yield invariant {:layer 99} Yield_RootScanBarrierInv();
 invariant RootScanBarrierInv(mutatorsInRootScanBarrier, rootScanBarrier);
 
-yield invariant {:layer 99} Yield_InitVars99({:linear "tid"} mutatorTids:[int]bool, tick_mutatorsInRootScanBarrier: [int]bool, tick_rootScanBarrier: int);
-invariant (forall i:int :: mutatorId(i) ==> mutatorTids[i] && mutatorTids[-i]);
+yield invariant {:layer 99} Yield_InitVars99({:linear} mutatorTids:Set Piece, tick_mutatorsInRootScanBarrier: Set Piece, tick_rootScanBarrier: int);
+invariant (forall i:int :: mutatorId(i) ==> Set_Contains(mutatorTids, Left(i)) && Set_Contains(mutatorTids, Right(i)));
 invariant mutatorsInRootScanBarrier == tick_mutatorsInRootScanBarrier;
 invariant rootScanBarrier == tick_rootScanBarrier;
 
-yield invariant {:layer 99} Yield_RootScanOn({:linear "tid"} tid: Tid, tick_rootScanOn: bool);
+yield invariant {:layer 99} Yield_RootScanOn({:linear} tid: Tid, tick_rootScanOn: bool);
 invariant tid == GcTid;
 invariant rootScanOn == tick_rootScanOn;
 
-yield invariant {:layer 99} Yield_RootScanBarrierEnter({:linear "tid"} tid: Tid);
+yield invariant {:layer 99} Yield_RootScanBarrierEnter({:linear} tid: Tid);
 invariant mutatorTidWhole(tid);
-invariant !mutatorsInRootScanBarrier[tid->i];
+invariant !Set_Contains(mutatorsInRootScanBarrier, Right(tid->i));
 
-yield invariant {:layer 99} Yield_RootScanBarrierWait({:linear "tid"} tid: Tid);
+yield invariant {:layer 99} Yield_RootScanBarrierWait({:linear} tid: Tid);
 invariant mutatorTidLeft(tid);
-invariant mutatorsInRootScanBarrier[tid->i];
+invariant Set_Contains(mutatorsInRootScanBarrier, Right(tid->i));
 
 yield procedure {:layer 99}
-InitVars99({:layer 95, 99} {:linear "tid"} tid:Tid, {:layer 95, 99} {:linear "tid"} mutatorTids:[int]bool)
+InitVars99({:layer 95, 99} {:linear} tid:Tid, {:layer 95, 99} {:linear} mutatorTids:Set Piece)
 requires {:layer 98,99} gcAndMutatorTids(tid, mutatorTids);
 ensures call Yield_InitVars98(tid, mutatorTids, 0);
 requires call Yield_InitVars99(mutatorTids, old(mutatorsInRootScanBarrier), old(rootScanBarrier));
@@ -542,29 +531,29 @@ ensures call Yield_InitVars99(mutatorTids, old(mutatorsInRootScanBarrier), numMu
 }
 
 yield procedure {:layer 99}
-TestRootScanBarrier({:layer 95, 99} {:linear "tid"} tid:Tid)
+TestRootScanBarrier({:layer 95, 99} {:linear} tid:Tid)
 requires {:layer 95,96} mutatorTidWhole(tid);
 requires call Yield_RootScanBarrierEnter(tid);
 requires call Yield_RootScanBarrierInv();
 preserves call Yield_Lock();
 {
     var isRootScanOn: bool;
-    var {:layer 95, 99} {:linear "tid"} tid_tmp: Tid;
+    var {:layer 95, 99} {:linear} tid_tmp: Tid;
 
     par isRootScanOn := PollMutatorReadBarrierOn(tid) | Yield_Lock();
     par Yield_RootScanBarrierInv() | Yield_RootScanBarrierEnter(tid) | Yield_97() | Yield_98();
     if (isRootScanOn)
     {
-        assert{:layer 99} mutatorsInRootScanBarrier == mutatorsInRootScanBarrier[tid->i := false];
+        assert{:layer 99} !Set_Contains(mutatorsInRootScanBarrier, Right(tid->i));
         call tid_tmp := MutatorRootScanBarrierEnter(tid);
         par Yield_RootScanBarrierInv() | Yield_RootScanBarrierWait(tid_tmp) | Yield_97() | Yield_98();
-        assert{:layer 99} mutatorsInRootScanBarrier == mutatorsInRootScanBarrier[tid_tmp->i := true];
+        assert{:layer 99} Set_Contains(mutatorsInRootScanBarrier, Right(tid_tmp->i));
         call tid_tmp := MutatorRootScanBarrierWait(tid_tmp);
-        call {:layer 95, 99} TidOutput(tid_tmp, tid);
+        call {:layer 99} Move(tid_tmp, tid);
     }
 }
 
-atomic action {:layer 100} AtomicCanMarkStop({:linear "tid"} tid:Tid) returns (canStop: bool)
+atomic action {:layer 100} AtomicCanMarkStop({:linear} tid:Tid) returns (canStop: bool)
 modifies Color;
 {
     assert tid == GcTid;
@@ -574,7 +563,7 @@ modifies Color;
 }
 
 yield procedure {:layer 99}
-CanMarkStop({:layer 95, 99} {:linear "tid"} tid:Tid) returns (canStop: bool)
+CanMarkStop({:layer 95, 99} {:linear} tid:Tid) returns (canStop: bool)
 refines AtomicCanMarkStop;
 requires {:layer 99} tid == GcTid;
 preserves call Yield_MsWellFormed(tid, 0);
@@ -614,7 +603,7 @@ preserves call Yield_Lock();
     call CollectorRootScanBarrierEnd(tid);
 }
 
-atomic action {:layer 100} AtomicWriteFieldRaw({:linear "tid"} tid:Tid, x: idx, f: fld, y: idx)
+atomic action {:layer 100} AtomicWriteFieldRaw({:linear} tid:Tid, x: idx, f: fld, y: idx)
 modifies memAbs,  mem;
 {
     assert mutatorTidWhole(tid) && rootAddr(x) && tidOwns(tid, x) && fieldAddr(f) && rootAddr(y) && tidOwns(tid, y) && memAddr(root[x]) && toAbs[root[x]] != nil && memAddrAbs(rootAbs[x]);
@@ -622,7 +611,7 @@ modifies memAbs,  mem;
     mem[root[x]][f] := root[y];
 }
 
-yield procedure {:layer 99} WriteFieldRaw({:layer 95, 99} {:linear "tid"} tid:Tid, x: idx, f: fld, y: idx)
+yield procedure {:layer 99} WriteFieldRaw({:layer 95, 99} {:linear} tid:Tid, x: idx, f: fld, y: idx)
 refines AtomicWriteFieldRaw;
 requires {:layer 98} mutatorTidWhole(tid);
 {
@@ -635,7 +624,7 @@ requires {:layer 98} mutatorTidWhole(tid);
     call {:layer 99} memAbs := Copy((var a, b := rootAbs[x], rootAbs[y]; memAbs[a := memAbs[a][f := b]]));
 }
 
-atomic action {:layer 100} AtomicReadFieldRaw({:linear "tid"} tid:Tid, x: idx, f: fld, y: idx)
+atomic action {:layer 100} AtomicReadFieldRaw({:linear} tid:Tid, x: idx, f: fld, y: idx)
 modifies rootAbs, root;
 {
     assert mutatorTidWhole(tid) && rootAddr(x) && tidOwns(tid, x) && fieldAddr(f) && rootAddr(y) && tidOwns(tid, y) && memAddr(root[x]) && toAbs[root[x]] != nil && memAddrAbs(rootAbs[x]);
@@ -643,7 +632,7 @@ modifies rootAbs, root;
     root[y] := mem[root[x]][f];
 }
 
-yield procedure {:layer 99} ReadFieldRaw({:layer 95, 99} {:linear "tid"} tid:Tid, x: idx, f: fld, y: idx)
+yield procedure {:layer 99} ReadFieldRaw({:layer 95, 99} {:linear} tid:Tid, x: idx, f: fld, y: idx)
 refines AtomicReadFieldRaw;
 {
     var valx: int;
@@ -655,10 +644,10 @@ refines AtomicReadFieldRaw;
     call {:layer 99} rootAbs := Copy((var a := rootAbs[x]; rootAbs[y := memAbs[a][f]]));
 }
 
-atomic action {:layer 100} AtomicEqRaw({:linear "tid"} tid:Tid, x: idx, y:idx) returns (isEqual:bool)
+atomic action {:layer 100} AtomicEqRaw({:linear} tid:Tid, x: idx, y:idx) returns (isEqual:bool)
 { assert mutatorTidWhole(tid) && rootAddr(x) && tidOwns(tid, x) && rootAddr(y) && tidOwns(tid, y); isEqual := root[x] == root[y]; }
 
-yield procedure {:layer 99} EqRaw({:layer 95, 99} {:linear "tid"} tid:Tid, x: idx, y:idx) returns (isEqual:bool)
+yield procedure {:layer 99} EqRaw({:layer 95, 99} {:linear} tid:Tid, x: idx, y:idx) returns (isEqual:bool)
 refines AtomicEqRaw;
 {
     var vx:int;
@@ -669,7 +658,7 @@ refines AtomicEqRaw;
     isEqual := vx == vy;
 }
 
-atomic action {:layer 100} AtomicAllocRaw({:linear "tid"} tid:Tid, y:idx) returns (ptr: int, absPtr: obj)
+atomic action {:layer 100} AtomicAllocRaw({:linear} tid:Tid, y:idx) returns (ptr: int, absPtr: obj)
 modifies allocSet, rootAbs, root, toAbs, memAbs, Color, mem;
 {
     assert mutatorTidWhole(tid) && rootAddr(y) && tidOwns(tid, y);
@@ -685,7 +674,7 @@ modifies allocSet, rootAbs, root, toAbs, memAbs, Color, mem;
     mem[ptr] := (lambda z: int :: if (fieldAddr(z)) then ptr else mem[ptr][z]);
 }
 
-yield procedure {:layer 99} AllocRaw({:layer 95, 99} {:linear "tid"} tid:Tid, y:idx) returns (ptr: int, absPtr: obj)
+yield procedure {:layer 99} AllocRaw({:layer 95, 99} {:linear} tid:Tid, y:idx) returns (ptr: int, absPtr: obj)
 refines AtomicAllocRaw;
 preserves call Yield_Lock();
 {
@@ -697,7 +686,7 @@ preserves call Yield_Lock();
     call {:layer 99} rootAbs := Copy(rootAbs[y := absPtr]);
 }
 
-atomic action {:layer 100} AtomicWriteBarrier({:linear "tid"} tid:Tid, i: int, y:idx)
+atomic action {:layer 100} AtomicWriteBarrier({:linear} tid:Tid, i: int, y:idx)
 modifies Color;
 {
     var val:int;
@@ -708,7 +697,7 @@ modifies Color;
     }
 }
 
-yield procedure {:layer 99} WriteBarrier({:layer 95, 99} {:linear "tid"} tid:Tid, i: int, y:idx)
+yield procedure {:layer 99} WriteBarrier({:layer 95, 99} {:linear} tid:Tid, i: int, y:idx)
 refines AtomicWriteBarrier;
 requires {:layer 98} mutatorTidWhole(tid);
 requires {:layer 96,99} tid->i == i;
@@ -732,37 +721,37 @@ preserves call Yield_Lock();
 // Layer 98
 //////////////////////////////////////////////////////////////////////////////
 
-yield invariant {:layer 98} Yield_MsWellFormed({:linear "tid"} tid:Tid, nodePeeked: int);
+yield invariant {:layer 98} Yield_MsWellFormed({:linear} tid:Tid, nodePeeked: int);
 invariant tid == GcTid;
 invariant MsWellFormed(MarkStack, MarkStackPtr, Color, nodePeeked);
 
-yield invariant {:layer 98} Yield_CollectorPhase_98({:linear "tid"} tid:Tid, tick_collectorPhase: int);
+yield invariant {:layer 98} Yield_CollectorPhase_98({:linear} tid:Tid, tick_collectorPhase: int);
 invariant tid == GcTid;
 invariant tick_collectorPhase == collectorPhase;
 
-yield invariant {:layer 98} Yield_SweepPtr_98({:linear "tid"} tid:Tid, tick_sweepPtr: int);
+yield invariant {:layer 98} Yield_SweepPtr_98({:linear} tid:Tid, tick_sweepPtr: int);
 invariant tid == GcTid;
 invariant tick_sweepPtr == sweepPtr;
 
-yield invariant {:layer 98} Yield_MarkPhase({:linear "tid"} tid:Tid, ptr: int);
+yield invariant {:layer 98} Yield_MarkPhase({:linear} tid:Tid, ptr: int);
 invariant mutatorTidWhole(tid);
 invariant MarkPhase(mutatorPhase[tid->i]);
 
 yield invariant {:layer 98} Yield_98();
 
-yield invariant {:layer 98} Yield_InitVars98({:linear "tid"} tid:Tid, {:linear "tid"} mutatorTids:[int]bool, tick_MarkStackPtr: int);
+yield invariant {:layer 98} Yield_InitVars98({:linear} tid:Tid, {:linear} mutatorTids:Set Piece, tick_MarkStackPtr: int);
 invariant gcAndMutatorTids(tid, mutatorTids);
 invariant MarkStackPtr == tick_MarkStackPtr;
 
 yield procedure {:layer 98}
-InitVars98({:layer 95, 98} {:linear "tid"} tid:Tid, {:layer 95, 98} {:linear "tid"} mutatorTids:[int]bool)
+InitVars98({:layer 95, 98} {:linear} tid:Tid, {:layer 95, 98} {:linear} mutatorTids:Set Piece)
 requires call Yield_InitVars98(tid, mutatorTids, old(MarkStackPtr));
 ensures call Yield_InitVars98(tid, mutatorTids, 0);
 {
     call InitMarkStackPtr(tid, mutatorTids);
 }
 
-atomic action {:layer 99} AtomicFindFreePtr({:linear "tid"} tid: Tid, absPtr: obj) returns (ptr: int)
+atomic action {:layer 99} AtomicFindFreePtr({:linear} tid: Tid, absPtr: obj) returns (ptr: int)
 modifies Color, toAbs, mem;
 {
     assert mutatorTidWhole(tid);
@@ -773,7 +762,7 @@ modifies Color, toAbs, mem;
     mem[ptr] := (lambda z: int :: if (fieldAddr(z)) then ptr else mem[ptr][z]);
 }
 
-yield procedure {:layer 98} FindFreePtr({:layer 95, 98} {:linear "tid"} tid: Tid, absPtr: obj) returns (ptr: int)
+yield procedure {:layer 98} FindFreePtr({:layer 95, 98} {:linear} tid: Tid, absPtr: obj) returns (ptr: int)
 refines AtomicFindFreePtr;
 preserves call Yield_Lock();
 {
@@ -807,7 +796,7 @@ preserves call Yield_Lock();
     }
 }
 
-atomic action {:layer 99} AtomicInsertIntoSetIfWhiteByMutator({:linear "tid"} tid:Tid, memLocal:int)
+atomic action {:layer 99} AtomicInsertIntoSetIfWhiteByMutator({:linear} tid:Tid, memLocal:int)
 modifies Color;
 {
     assert mutatorTidWhole(tid) && memAddr(memLocal) && MarkPhase(mutatorPhase[tid->i]);
@@ -817,7 +806,7 @@ modifies Color;
 }
 
 yield procedure {:layer 98}
-InsertIntoSetIfWhiteByMutator({:layer 95, 98} {:linear "tid"} tid:Tid, memLocal:int)
+InsertIntoSetIfWhiteByMutator({:layer 95, 98} {:linear} tid:Tid, memLocal:int)
 refines AtomicInsertIntoSetIfWhiteByMutator;
 preserves call Yield_MarkPhase(tid, memLocal);
 preserves call Yield_Lock();
@@ -836,14 +825,14 @@ preserves call Yield_Lock();
     assert {:layer 98} MST(MarkStackPtr-1);
 }
 
-left action {:layer 99} AtomicNoGrayInRootScanBarrier({:linear "tid"} tid:Tid) returns (noGray: bool)
+left action {:layer 99} AtomicNoGrayInRootScanBarrier({:linear} tid:Tid) returns (noGray: bool)
 {
     assert tid == GcTid && rootScanOn && mutatorsInRootScanBarrier == Mutators;
     noGray := (forall i: int :: memAddr(i) ==> !Gray(Color[i]));
 }
 
 yield procedure {:layer 98}
-NoGrayInRootScanBarrier({:layer 95, 98} {:linear "tid"} tid:Tid) returns (noGray: bool)
+NoGrayInRootScanBarrier({:layer 95, 98} {:linear} tid:Tid) returns (noGray: bool)
 refines AtomicNoGrayInRootScanBarrier;
 preserves call Yield_MsWellFormed(tid, 0);
 preserves call Yield_CollectorPhase_98(tid, old(collectorPhase));
@@ -853,7 +842,7 @@ preserves call Yield_Lock();
     assert {:layer 98} noGray || MST(0);
 }
 
-left action {:layer 99} AtomicInsertIntoSetIfWhiteInRootScanBarrier({:linear "tid"} tid:Tid, memLocal:int)
+left action {:layer 99} AtomicInsertIntoSetIfWhiteInRootScanBarrier({:linear} tid:Tid, memLocal:int)
 modifies Color;
 {
     assert tid == GcTid && rootScanOn && mutatorsInRootScanBarrier == Mutators && memAddr(memLocal);
@@ -863,7 +852,7 @@ modifies Color;
 }
 
 yield procedure {:layer 98}
-InsertIntoSetIfWhiteInRootScanBarrier({:layer 95, 98} {:linear "tid"} tid:Tid, memLocal:int)
+InsertIntoSetIfWhiteInRootScanBarrier({:layer 95, 98} {:linear} tid:Tid, memLocal:int)
 refines AtomicInsertIntoSetIfWhiteInRootScanBarrier;
 preserves call Yield_MsWellFormed(tid, 0);
 preserves call Yield_CollectorPhase_98(tid, old(collectorPhase));
@@ -873,7 +862,7 @@ preserves call Yield_Lock();
     assert {:layer 98} MST(MarkStackPtr-1);
 }
 
-left action {:layer 99,100} AtomicInsertIntoSetIfWhiteByCollector({:linear "tid"} tid:Tid, parent: int, child:int)
+left action {:layer 99,100} AtomicInsertIntoSetIfWhiteByCollector({:linear} tid:Tid, parent: int, child:int)
 modifies Color;
 {
     assert tid == GcTid;
@@ -884,7 +873,7 @@ modifies Color;
 }
 
 yield procedure {:layer 98}
-InsertIntoSetIfWhiteByCollector({:layer 95, 98} {:linear "tid"} tid:Tid, parent: int, child:int)
+InsertIntoSetIfWhiteByCollector({:layer 95, 98} {:linear} tid:Tid, parent: int, child:int)
 refines AtomicInsertIntoSetIfWhiteByCollector;
 requires {:layer 98} memAddr(parent) && memAddr(child);
 preserves call Yield_MsWellFormed(tid, parent);
@@ -895,7 +884,7 @@ preserves call Yield_Lock();
     assert {:layer 98} MST(MarkStackPtr-1);
 }
 
-right action {:layer 99,100} AtomicRemoveFromStack({:linear "tid"} tid:Tid) returns (isEmpty: bool, val:int)
+right action {:layer 99,100} AtomicRemoveFromStack({:linear} tid:Tid) returns (isEmpty: bool, val:int)
 {
     assert tid == GcTid;
     assert MarkPhase(collectorPhase) && PhaseConsistent(collectorPhase, mutatorPhase);
@@ -908,7 +897,7 @@ right action {:layer 99,100} AtomicRemoveFromStack({:linear "tid"} tid:Tid) retu
 }
 
 yield procedure {:layer 98}
-RemoveFromStack({:layer 95, 98} {:linear "tid"} tid:Tid) returns (isEmpty: bool, val:int)
+RemoveFromStack({:layer 95, 98} {:linear} tid:Tid) returns (isEmpty: bool, val:int)
 refines AtomicRemoveFromStack;
 requires call Yield_MsWellFormed(tid, 0);
 ensures call Yield_MsWellFormed(tid, if isEmpty then 0 else val);
@@ -925,19 +914,19 @@ preserves call Yield_Lock();
 
 yield invariant {:layer 97} Yield_97();
 
-yield invariant {:layer 97} Yield_WaitForMutators({:linear "tid"} tid:Tid, nextPhase: int, done: bool, i: int);
+yield invariant {:layer 97} Yield_WaitForMutators({:linear} tid:Tid, nextPhase: int, done: bool, i: int);
 invariant tid == GcTid;
 invariant nextPhase == collectorPhase;
 invariant done ==> (forall j:int:: 1 <= j && j < i ==> nextPhase == mutatorPhase[j]);
 
-atomic action {:layer 98,100} AtomicWaitForMutators({:linear "tid"} tid:Tid, nextPhase: int)
+atomic action {:layer 98,100} AtomicWaitForMutators({:linear} tid:Tid, nextPhase: int)
 {
     assert tid == GcTid;
     assume (forall j:int:: mutatorId(j) ==> nextPhase == mutatorPhase[j]);
 }
 
 yield procedure {:layer 97}
-WaitForMutators({:layer 95, 97} {:linear "tid"} tid:Tid, nextPhase: int)
+WaitForMutators({:layer 95, 97} {:linear} tid:Tid, nextPhase: int)
 refines AtomicWaitForMutators;
 requires call Yield_WaitForMutators(tid, nextPhase, false, 0);
 {
@@ -972,11 +961,11 @@ requires call Yield_WaitForMutators(tid, nextPhase, false, 0);
 // Layer 96
 //////////////////////////////////////////////////////////////////////////////
 
-atomic action {:layer 97,100} AtomicInitVars100({:linear "tid"} tid:Tid, {:linear "tid"} mutatorTids:[int]bool)
+atomic action {:layer 97,100} AtomicInitVars100({:linear} tid:Tid, {:linear} mutatorTids:Set Piece)
 modifies mutatorPhase, root, toAbs, Color, mem, collectorPhase, sweepPtr;
 {
     assert tid == GcTid;
-    assert (forall i:int :: mutatorId(i) ==> mutatorTids[i] && mutatorTids[-i]);
+    assert (forall i:int :: mutatorId(i) ==> Set_Contains(mutatorTids, Left(i)) && Set_Contains(mutatorTids, Right(i)));
     havoc mem, root, Color, mutatorPhase;
     assume (forall x: int, f: fld :: memAddr(x) && fieldAddr(f) ==> mem[x][f] == x);
     assume (forall x: idx :: rootAddr(x) ==> root[x] == 0);
@@ -987,7 +976,7 @@ modifies mutatorPhase, root, toAbs, Color, mem, collectorPhase, sweepPtr;
     sweepPtr := memHi;
 }
 
-yield procedure {:layer 96} InitVars100({:layer 95, 96} {:linear "tid"} tid:Tid, {:layer 95, 96} {:linear "tid"} mutatorTids:[int]bool)
+yield procedure {:layer 96} InitVars100({:layer 95, 96} {:linear} tid:Tid, {:layer 95, 96} {:linear} mutatorTids:Set Piece)
 refines AtomicInitVars100;
 {
     var n:int;
@@ -1049,7 +1038,7 @@ refines AtomicInitVars100;
     call InitSweepPtr(tid, mutatorTids);
 }
 
-atomic action {:layer 97,100} AtomicSetColorToBlack({:linear "tid"} tid:Tid, scannedLocal:int)
+atomic action {:layer 97,100} AtomicSetColorToBlack({:linear} tid:Tid, scannedLocal:int)
 modifies Color;
 {
     assert MarkPhase(collectorPhase) && PhaseConsistent(collectorPhase, mutatorPhase);
@@ -1058,7 +1047,7 @@ modifies Color;
     Color[scannedLocal] := BLACK();
 }
 
-yield procedure {:layer 96} SetColorToBlack({:layer 95, 96} {:linear "tid"} tid:Tid, scannedLocal:int)
+yield procedure {:layer 96} SetColorToBlack({:layer 95, 96} {:linear} tid:Tid, scannedLocal:int)
 refines AtomicSetColorToBlack;
 preserves call Yield_Lock();
 {
@@ -1067,7 +1056,7 @@ preserves call Yield_Lock();
     call LockRelease(tid);
 }
 
-atomic action {:layer 97,98} AtomicMsPushByCollector({:linear "tid"} tid: Tid, val: int)
+atomic action {:layer 97,98} AtomicMsPushByCollector({:linear} tid: Tid, val: int)
 modifies Color, MarkStack, MarkStackPtr;
 {
     assert memAddr(val) && tid == GcTid;
@@ -1078,7 +1067,7 @@ modifies Color, MarkStack, MarkStackPtr;
     }
 }
 
-yield procedure {:layer 96} MsPushByCollector({:layer 95, 96} {:linear "tid"} tid: Tid, val: int)
+yield procedure {:layer 96} MsPushByCollector({:layer 95, 96} {:linear} tid: Tid, val: int)
 refines AtomicMsPushByCollector;
 preserves call Yield_Lock();
 {
@@ -1098,7 +1087,7 @@ preserves call Yield_Lock();
     call LockRelease(tid);
 }
 
-atomic action {:layer 97,98} AtomicMsPushByMutator({:linear "tid"} tid: Tid, val: int)
+atomic action {:layer 97,98} AtomicMsPushByMutator({:linear} tid: Tid, val: int)
 modifies Color, MarkStack, MarkStackPtr;
 {
     assert memAddr(val) && mutatorTidWhole(tid) && MarkPhase(mutatorPhase[tid->i]);
@@ -1109,7 +1098,7 @@ modifies Color, MarkStack, MarkStackPtr;
     }
 }
 
-yield procedure {:layer 96} MsPushByMutator({:layer 95, 96} {:linear "tid"} tid: Tid, val: int)
+yield procedure {:layer 96} MsPushByMutator({:layer 95, 96} {:linear} tid: Tid, val: int)
 refines AtomicMsPushByMutator;
 preserves call Yield_Lock();
 {
@@ -1129,7 +1118,7 @@ preserves call Yield_Lock();
     call LockRelease(tid);
 }
 
-atomic action {:layer 97,98} AtomicMsPop({:linear "tid"} tid:Tid) returns (isEmpty: bool, val:int)
+atomic action {:layer 97,98} AtomicMsPop({:linear} tid:Tid) returns (isEmpty: bool, val:int)
 modifies MarkStackPtr;
 {
     assert tid == GcTid;
@@ -1143,7 +1132,7 @@ modifies MarkStackPtr;
     }
 }
 
-yield procedure {:layer 96} MsPop({:layer 95, 96} {:linear "tid"} tid:Tid) returns (isEmpty: bool, val:int)
+yield procedure {:layer 96} MsPop({:layer 95, 96} {:linear} tid:Tid) returns (isEmpty: bool, val:int)
 refines AtomicMsPop;
 preserves call Yield_Lock();
 {
@@ -1166,10 +1155,10 @@ preserves call Yield_Lock();
     call LockRelease(tid);
 }
 
-atomic action {:layer 97,98} AtomicMsIsEmpty({:linear "tid"} tid: Tid) returns (isEmpty: bool)
+atomic action {:layer 97,98} AtomicMsIsEmpty({:linear} tid: Tid) returns (isEmpty: bool)
 { assert tid == GcTid; isEmpty := MarkStackPtr == 0; }
 
-yield procedure {:layer 96} MsIsEmpty({:layer 95, 96} {:linear "tid"} tid: Tid) returns (isEmpty: bool)
+yield procedure {:layer 96} MsIsEmpty({:layer 95, 96} {:linear} tid: Tid) returns (isEmpty: bool)
 refines AtomicMsIsEmpty;
 preserves call Yield_Lock();
 {
@@ -1181,11 +1170,11 @@ preserves call Yield_Lock();
     call LockRelease(tid);
 }
 
-atomic action {:layer 97,100} AtomicResetSweepPtr({:linear "tid"} tid:Tid)
+atomic action {:layer 97,100} AtomicResetSweepPtr({:linear} tid:Tid)
 modifies sweepPtr;
 { assert tid == GcTid; sweepPtr := memLo; }
 
-yield procedure {:layer 96} ResetSweepPtr({:layer 95, 96} {:linear "tid"} tid:Tid)
+yield procedure {:layer 96} ResetSweepPtr({:layer 95, 96} {:linear} tid:Tid)
 refines AtomicResetSweepPtr;
 preserves call Yield_Lock();
 {
@@ -1194,7 +1183,7 @@ preserves call Yield_Lock();
     call LockRelease(tid);
 }
 
-left action {:layer 97,100} AtomicSweepNext({:linear "tid"} tid:Tid)
+left action {:layer 97,100} AtomicSweepNext({:linear} tid:Tid)
 modifies Color, sweepPtr;
 {
     assert SweepPhase(collectorPhase) && PhaseConsistent(collectorPhase, mutatorPhase);
@@ -1205,7 +1194,7 @@ modifies Color, sweepPtr;
     sweepPtr := sweepPtr + 1;
 }
 
-yield procedure {:layer 96} SweepNext({:layer 95, 96} {:linear "tid"} tid:Tid)
+yield procedure {:layer 96} SweepNext({:layer 95, 96} {:linear} tid:Tid)
 refines AtomicSweepNext;
 preserves call Yield_Lock();
 {
@@ -1222,7 +1211,7 @@ preserves call Yield_Lock();
     call LockRelease(tid);
 }
 
-atomic action {:layer 97,100} AtomicHandshakeCollector({:linear "tid"} tid:Tid) returns (nextPhase: int)
+atomic action {:layer 97,100} AtomicHandshakeCollector({:linear} tid:Tid) returns (nextPhase: int)
 modifies collectorPhase;
 {
     assert tid == GcTid;
@@ -1239,7 +1228,7 @@ modifies collectorPhase;
     }
 }
 
-yield procedure {:layer 96} HandshakeCollector({:layer 95, 96} {:linear "tid"} tid:Tid) returns (nextPhase: int)
+yield procedure {:layer 96} HandshakeCollector({:layer 95, 96} {:linear} tid:Tid) returns (nextPhase: int)
 refines AtomicHandshakeCollector;
 preserves call Yield_Lock();
 {
@@ -1252,11 +1241,11 @@ preserves call Yield_Lock();
     call LockRelease(tid);
 }
 
-atomic action {:layer 97,100} AtomicUpdateMutatorPhase({:linear "tid"} tid: Tid, i: int)
+atomic action {:layer 97,100} AtomicUpdateMutatorPhase({:linear} tid: Tid, i: int)
 modifies mutatorPhase;
 { assert mutatorTidWhole(tid); mutatorPhase[tid->i] := collectorPhase; }
 
-yield procedure {:layer 96} UpdateMutatorPhase({:layer 95, 96} {:linear "tid"} tid: Tid, i: int)
+yield procedure {:layer 96} UpdateMutatorPhase({:layer 95, 96} {:linear} tid: Tid, i: int)
 refines AtomicUpdateMutatorPhase;
 preserves call Yield_Lock();
 requires {:layer 96} tid->i == i;
@@ -1269,11 +1258,11 @@ requires {:layer 96} tid->i == i;
     call LockRelease(tid);
 }
 
-atomic action {:layer 97,99} AtomicCollectorRootScanBarrierStart({:linear "tid"} tid: Tid)
+atomic action {:layer 97,99} AtomicCollectorRootScanBarrierStart({:linear} tid: Tid)
 modifies rootScanOn;
 { assert tid == GcTid; rootScanOn := true; }
 
-yield procedure {:layer 96} CollectorRootScanBarrierStart({:layer 95, 96} {:linear "tid"} tid: Tid)
+yield procedure {:layer 96} CollectorRootScanBarrierStart({:layer 95, 96} {:linear} tid: Tid)
 refines AtomicCollectorRootScanBarrierStart;
 preserves call Yield_Lock();
 {
@@ -1282,11 +1271,11 @@ preserves call Yield_Lock();
     call LockRelease(tid);
 }
 
-left action {:layer 97,99} AtomicCollectorRootScanBarrierEnd({:linear "tid"} tid: Tid)
+left action {:layer 97,99} AtomicCollectorRootScanBarrierEnd({:linear} tid: Tid)
 modifies rootScanOn;
 { assert tid == GcTid; rootScanOn := false; }
 
-yield procedure {:layer 96} CollectorRootScanBarrierEnd({:layer 95, 96} {:linear "tid"} tid: Tid)
+yield procedure {:layer 96} CollectorRootScanBarrierEnd({:layer 95, 96} {:linear} tid: Tid)
 refines AtomicCollectorRootScanBarrierEnd;
 preserves call Yield_Lock();
 {
@@ -1295,10 +1284,10 @@ preserves call Yield_Lock();
     call LockRelease(tid);
 }
 
-atomic action {:layer 97,99} AtomicCollectorRootScanBarrierWait({:linear "tid"} tid: Tid)
+atomic action {:layer 97,99} AtomicCollectorRootScanBarrierWait({:linear} tid: Tid)
 { assert tid == GcTid; assume rootScanBarrier == 0; }
 
-yield procedure {:layer 96} CollectorRootScanBarrierWait({:layer 95, 96} {:linear "tid"} tid: Tid)
+yield procedure {:layer 96} CollectorRootScanBarrierWait({:layer 95, 96} {:linear} tid: Tid)
 refines AtomicCollectorRootScanBarrierWait;
 {
     var v:int;
@@ -1314,22 +1303,24 @@ refines AtomicCollectorRootScanBarrierWait;
     }
 }
 
-atomic action {:layer 97,99} AtomicMutatorRootScanBarrierEnter({:linear_in "tid"} tid: Tid) returns({:linear "tid"} tid_left: Tid)
+atomic action {:layer 97,99} AtomicMutatorRootScanBarrierEnter({:linear_in} tid: Tid) returns({:linear} tid_left: Tid)
 modifies rootScanBarrier, mutatorsInRootScanBarrier;
 {
+    var {:linear} p: One Piece;
     assert mutatorTidWhole(tid);
     rootScanBarrier := rootScanBarrier - 1;
-    mutatorsInRootScanBarrier[tid->i] := true;
-    tid_left := Tid(tid->i, true, false);
+    tid_left := tid;
+    call p := One_Get(tid_left->ps, Right(tid_left->i));
+    call One_Put(mutatorsInRootScanBarrier, p);
 }
 
-yield procedure {:layer 96} MutatorRootScanBarrierEnter({:layer 95, 96} {:linear_in "tid"} tid: Tid) returns({:layer 95, 96} {:linear "tid"} tid_left: Tid)
+yield procedure {:layer 96} MutatorRootScanBarrierEnter({:layer 95, 96} {:linear_in} tid: Tid) returns({:layer 95, 96} {:linear} tid_left: Tid)
 refines AtomicMutatorRootScanBarrierEnter;
 requires {:layer 95} mutatorTidWhole(tid);
-ensures {:layer 95,96} tid_left->i == tid->i && tid_left->left;
+ensures {:layer 95,96} mutatorTidLeft(tid_left);
 preserves call Yield_Lock();
 {
-    var {:layer 95, 96} {:linear "tid"} tid_right: Tid;
+    var {:layer 95, 96} {:linear} tid_right: Tid;
 
     call {:layer 95, 96} tid_left, tid_right := TidSplit(tid);
     call LockAcquire(tid_left);
@@ -1338,22 +1329,26 @@ preserves call Yield_Lock();
     call LockRelease(tid_left);
 }
 
-atomic action {:layer 97,99} AtomicMutatorRootScanBarrierWait({:linear_in "tid"} tid_left: Tid) returns({:linear "tid"} tid: Tid)
+atomic action {:layer 97,99} AtomicMutatorRootScanBarrierWait({:linear_in} tid_left: Tid) returns({:linear} tid: Tid)
 modifies rootScanBarrier, mutatorsInRootScanBarrier;
 {
-    assert mutatorTidLeft(tid_left) && mutatorsInRootScanBarrier[tid_left->i];
+    var {:linear} p: One Piece; 
+    assert mutatorTidLeft(tid_left) && Set_Contains(mutatorsInRootScanBarrier, Right(tid_left->i));
     assume !rootScanOn;
     rootScanBarrier := rootScanBarrier + 1;
-    mutatorsInRootScanBarrier[tid_left->i] := false;
-    tid := Tid(tid_left->i, true, true);
+    call p := One_Get(mutatorsInRootScanBarrier, Right(tid_left->i));
+    tid := tid_left;
+    call One_Put(tid->ps, p);
 }
 
-yield procedure {:layer 96} MutatorRootScanBarrierWait({:layer 95, 96} {:linear_in "tid"} tid_left: Tid) returns({:layer 95, 96} {:linear "tid"} tid: Tid)
+yield procedure {:layer 96} MutatorRootScanBarrierWait({:layer 95, 96} {:linear_in} tid_left: Tid) returns({:layer 95, 96} {:linear} tid: Tid)
 refines AtomicMutatorRootScanBarrierWait;
-ensures {:layer 95,96} tid->i == tid_left->i && tid->left && tid->right;
+requires {:layer 95,96} mutatorTidLeft(tid_left);
+ensures {:layer 95,96} tid->i == tid_left->i;
+ensures {:layer 95,96} mutatorTidWhole(tid);
 preserves call Yield_Lock();
 {
-    var {:layer 95, 96} {:linear "tid"} tid_right: Tid;
+    var {:layer 95, 96} {:linear} tid_right: Tid;
     var b: bool;
 
     loop:
@@ -1373,7 +1368,7 @@ preserves call Yield_Lock();
         goto loop;
 }
 
-atomic action {:layer 97,98} AtomicAllocIfPtrFree({:linear "tid"} tid:Tid, ptr:int, absPtr:obj) returns (spaceFound:bool)
+atomic action {:layer 97,98} AtomicAllocIfPtrFree({:linear} tid:Tid, ptr:int, absPtr:obj) returns (spaceFound:bool)
 modifies Color, toAbs, mem;
 {
     assert mutatorTidWhole(tid) && memAddr(ptr) && (Unalloc(Color[ptr]) ==> toAbs[ptr] == nil);
@@ -1388,7 +1383,7 @@ modifies Color, toAbs, mem;
     }
 }
 
-yield procedure {:layer 96} AllocIfPtrFree({:layer 95, 96} {:linear "tid"} tid:Tid, ptr:int, absPtr:obj) returns (spaceFound:bool)
+yield procedure {:layer 96} AllocIfPtrFree({:layer 95, 96} {:linear} tid:Tid, ptr:int, absPtr:obj) returns (spaceFound:bool)
 refines AtomicAllocIfPtrFree;
 preserves call Yield_Lock();
 {
@@ -1438,10 +1433,10 @@ preserves call Yield_Lock();
     spaceFound := false;
 }
 
-atomic action {:layer 97,100} AtomicIsWhiteByCollector({:linear "tid"} tid:Tid, i: int) returns (isWhite: bool)
+atomic action {:layer 97,100} AtomicIsWhiteByCollector({:linear} tid:Tid, i: int) returns (isWhite: bool)
 { assert tid == GcTid && memAddr(i); isWhite := White(Color[i]); }
 
-yield procedure {:layer 96} IsWhiteByCollector({:layer 95, 96} {:linear "tid"} tid:Tid, i: int) returns (isWhite: bool)
+yield procedure {:layer 96} IsWhiteByCollector({:layer 95, 96} {:linear} tid:Tid, i: int) returns (isWhite: bool)
 refines AtomicIsWhiteByCollector;
 preserves call Yield_Lock();
 {
@@ -1453,11 +1448,11 @@ preserves call Yield_Lock();
     call LockRelease(tid);
 }
 
-atomic action {:layer 97,100} AtomicClearToAbsWhite({:linear "tid"} tid:Tid)
+atomic action {:layer 97,100} AtomicClearToAbsWhite({:linear} tid:Tid)
 modifies toAbs;
 { assert tid == GcTid; toAbs := (lambda x: int :: if memAddr(x) && White(Color[x]) then nil else toAbs[x]); }
 
-yield procedure {:layer 96} ClearToAbsWhite({:layer 95, 96} {:linear "tid"} tid:Tid)
+yield procedure {:layer 96} ClearToAbsWhite({:layer 95, 96} {:linear} tid:Tid)
 refines AtomicClearToAbsWhite;
 preserves call Yield_Lock();
 {
@@ -1472,411 +1467,417 @@ yield invariant {:layer 96} Yield_96();
 // Layer 95
 //////////////////////////////////////////////////////////////////////////////
 
-atomic action {:layer 96} AtomicLockedClearToAbsWhite({:linear "tid"} tid:Tid)
+atomic action {:layer 96} AtomicLockedClearToAbsWhite({:linear} tid:Tid)
 modifies toAbs;
 { assert tid == GcTid && tidHasLock(tid, absLock); toAbs := (lambda x: int :: if memAddr(x) && White(Color[x]) then nil else toAbs[x]); }
 
-yield procedure {:layer 95} LockedClearToAbsWhite({:layer 95} {:linear "tid"} tid:Tid)
+yield procedure {:layer 95} LockedClearToAbsWhite({:layer 95} {:linear} tid:Tid)
 refines AtomicLockedClearToAbsWhite;
 {
     call {:layer 95} toAbs := Copy((lambda x: int :: if memAddr(x) && White(Color[x]) then nil else toAbs[x]));
 }
 
-both action {:layer 96,99} AtomicInitField({:linear "tid"} tid:Tid, {:linear "tid"} mutatorTids:[int]bool, x: int, f: int)
+both action {:layer 96,99} AtomicInitField({:linear} tid:Tid, {:linear} mutatorTids:Set Piece, x: int, f: int)
 modifies mem;
 { assert gcAndMutatorTids(tid, mutatorTids) && memAddr(x) && fieldAddr(f); mem[x][f] := x; }
 
-yield procedure {:layer 95} InitField({:layer 95} {:linear "tid"} tid:Tid, {:layer 95} {:linear "tid"} mutatorTids:[int]bool, x: int, f: int)
+yield procedure {:layer 95} InitField({:layer 95} {:linear} tid:Tid, {:layer 95} {:linear} mutatorTids:Set Piece, x: int, f: int)
 refines AtomicInitField;
 {
     call PrimitiveWriteField(x, f, x);
 }
 
-atomic action {:layer 96,100} AtomicReadFieldByCollector({:linear "tid"} tid:Tid, x:int, f: fld) returns (y: int)
+atomic action {:layer 96,100} AtomicReadFieldByCollector({:linear} tid:Tid, x:int, f: fld) returns (y: int)
 { assert tid == GcTid && memAddr(x) && fieldAddr(f) && toAbs[x] != nil; y := mem[x][f]; }
 
-yield procedure {:layer 95} ReadFieldByCollector({:layer 95} {:linear "tid"} tid:Tid, x:int, f: fld) returns (y: int)
+yield procedure {:layer 95} ReadFieldByCollector({:layer 95} {:linear} tid:Tid, x:int, f: fld) returns (y: int)
 refines AtomicReadFieldByCollector;
 {
     call y := PrimitiveReadField(x, f);
 }
 
-atomic action {:layer 96,99} AtomicReadFieldByMutator({:linear "tid"} tid:Tid, x: int, f: fld) returns (y: int)
+atomic action {:layer 96,99} AtomicReadFieldByMutator({:linear} tid:Tid, x: int, f: fld) returns (y: int)
 { assert mutatorTidWhole(tid) && memAddr(x) && fieldAddr(f) && toAbs[x] != nil; y := mem[x][f]; }
 
-yield procedure {:layer 95} ReadFieldByMutator({:layer 95} {:linear "tid"} tid:Tid, x: int, f: fld) returns (y: int)
+yield procedure {:layer 95} ReadFieldByMutator({:layer 95} {:linear} tid:Tid, x: int, f: fld) returns (y: int)
 refines AtomicReadFieldByMutator;
 {
     call y := PrimitiveReadField(x, f);
 }
 
-atomic action {:layer 96,99} AtomicWriteFieldByMutator({:linear "tid"} tid:Tid, x: int, f: fld, y: int)
+atomic action {:layer 96,99} AtomicWriteFieldByMutator({:linear} tid:Tid, x: int, f: fld, y: int)
 modifies mem;
 { assert mutatorTidWhole(tid) && memAddr(x) && fieldAddr(f) && toAbs[x] != nil; mem[x][f] := y; }
 
-yield procedure {:layer 95} WriteFieldByMutator({:layer 95} {:linear "tid"} tid:Tid, x: int, f: fld, y: int)
+yield procedure {:layer 95} WriteFieldByMutator({:layer 95} {:linear} tid:Tid, x: int, f: fld, y: int)
 refines AtomicWriteFieldByMutator;
 {
     call PrimitiveWriteField(x, f, y);
 }
 
-right action {:layer 96} AtomicInitializeFieldInAlloc({:linear "tid"} tid: Tid, ptr: int, fld: int)
+right action {:layer 96} AtomicInitializeFieldInAlloc({:linear} tid: Tid, ptr: int, fld: int)
 modifies mem;
 { assert mutatorTidWhole(tid) && tidHasLock(tid, absLock) && memAddr(ptr) && fieldAddr(fld) && toAbs[ptr] == nil; mem[ptr][fld] := ptr; }
 
-yield procedure {:layer 95} InitializeFieldInAlloc({:layer 95} {:linear "tid"} tid: Tid, ptr: int, fld: int)
+yield procedure {:layer 95} InitializeFieldInAlloc({:layer 95} {:linear} tid: Tid, ptr: int, fld: int)
 refines AtomicInitializeFieldInAlloc;
 {
     call PrimitiveWriteField(ptr, fld, ptr);
 }
 
-both action {:layer 96} AtomicReadMarkStackPtr({:linear "tid"} tid:Tid) returns (val: int)
+both action {:layer 96} AtomicReadMarkStackPtr({:linear} tid:Tid) returns (val: int)
 { assert tidHasLock(tid, absLock); val := MarkStackPtr; }
 
-yield procedure {:layer 95} ReadMarkStackPtr({:layer 95} {:linear "tid"} tid:Tid) returns (val: int)
+yield procedure {:layer 95} ReadMarkStackPtr({:layer 95} {:linear} tid:Tid) returns (val: int)
 refines AtomicReadMarkStackPtr;
 {
     call val := PrimitiveReadMarkStackPtr();
 }
 
-atomic action {:layer 96,98} AtomicInitMarkStackPtr({:linear "tid"} tid:Tid, {:linear "tid"} mutatorTids:[int]bool)
+atomic action {:layer 96,98} AtomicInitMarkStackPtr({:linear} tid:Tid, {:linear} mutatorTids:Set Piece)
 modifies MarkStackPtr;
 { assert gcAndMutatorTids(tid, mutatorTids); MarkStackPtr := 0; }
 
-yield procedure {:layer 95} InitMarkStackPtr({:layer 95} {:linear "tid"} tid:Tid, {:layer 95} {:linear "tid"} mutatorTids:[int]bool)
+yield procedure {:layer 95} InitMarkStackPtr({:layer 95} {:linear} tid:Tid, {:layer 95} {:linear} mutatorTids:Set Piece)
 refines AtomicInitMarkStackPtr;
 {
     call PrimitiveSetMarkStackPtr(0);
 }
 
-both action {:layer 96} AtomicSetMarkStackPtr({:linear "tid"} tid:Tid, val: int)
+both action {:layer 96} AtomicSetMarkStackPtr({:linear} tid:Tid, val: int)
 modifies MarkStackPtr;
 { assert tidHasLock(tid, absLock); MarkStackPtr := val; }
 
-yield procedure {:layer 95} SetMarkStackPtr({:layer 95} {:linear "tid"} tid:Tid, val: int)
+yield procedure {:layer 95} SetMarkStackPtr({:layer 95} {:linear} tid:Tid, val: int)
 refines AtomicSetMarkStackPtr;
 {
     call PrimitiveSetMarkStackPtr(val);
 }
 
-both action {:layer 96} AtomicReadMarkStack({:linear "tid"} tid:Tid, ptr: int) returns(val: int)
+both action {:layer 96} AtomicReadMarkStack({:linear} tid:Tid, ptr: int) returns(val: int)
 { assert tidHasLock(tid, absLock); val := MarkStack[ptr]; }
 
-yield procedure {:layer 95} ReadMarkStack({:layer 95} {:linear "tid"} tid:Tid, ptr: int) returns(val: int)
+yield procedure {:layer 95} ReadMarkStack({:layer 95} {:linear} tid:Tid, ptr: int) returns(val: int)
 refines AtomicReadMarkStack;
 {
     call val := PrimitiveReadMarkStack(ptr);
 }
 
-both action {:layer 96} AtomicWriteMarkStack({:linear "tid"} tid:Tid, ptr: int, val: int)
+both action {:layer 96} AtomicWriteMarkStack({:linear} tid:Tid, ptr: int, val: int)
 modifies MarkStack;
 { assert tidHasLock(tid, absLock); MarkStack[ptr] := val; }
 
-yield procedure {:layer 95} WriteMarkStack({:layer 95} {:linear "tid"} tid:Tid, ptr: int, val: int)
+yield procedure {:layer 95} WriteMarkStack({:layer 95} {:linear} tid:Tid, ptr: int, val: int)
 refines AtomicWriteMarkStack;
 {
     call PrimitiveWriteMarkStack(ptr, val);
 }
 
-both action {:layer 96,99} AtomicInitCollectorPhase({:linear "tid"} tid:Tid, {:linear "tid"} mutatorTids:[int]bool)
+both action {:layer 96,99} AtomicInitCollectorPhase({:linear} tid:Tid, {:linear} mutatorTids:Set Piece)
 modifies collectorPhase;
 { assert gcAndMutatorTids(tid, mutatorTids); collectorPhase := IDLE(); }
 
-yield procedure {:layer 95} InitCollectorPhase({:layer 95} {:linear "tid"} tid:Tid, {:layer 95} {:linear "tid"} mutatorTids:[int]bool)
+yield procedure {:layer 95} InitCollectorPhase({:layer 95} {:linear} tid:Tid, {:layer 95} {:linear} mutatorTids:Set Piece)
 refines AtomicInitCollectorPhase;
 {
     call PrimitiveSetCollectorPhase(IDLE());
 }
 
-atomic action {:layer 96} AtomicReadCollectorPhase({:linear "tid"} tid: Tid) returns (phase:int)
+atomic action {:layer 96} AtomicReadCollectorPhase({:linear} tid: Tid) returns (phase:int)
 { assert tid == GcTid; phase := collectorPhase; }
 
-yield procedure {:layer 95} ReadCollectorPhase({:layer 95} {:linear "tid"} tid: Tid) returns (phase:int)
+yield procedure {:layer 95} ReadCollectorPhase({:layer 95} {:linear} tid: Tid) returns (phase:int)
 refines AtomicReadCollectorPhase;
 {
     call phase := PrimitiveReadCollectorPhase();
 }
 
-right action {:layer 96} AtomicReadCollectorPhaseLocked({:linear "tid"} tid: Tid) returns (phase:int)
+right action {:layer 96} AtomicReadCollectorPhaseLocked({:linear} tid: Tid) returns (phase:int)
 { assert mutatorTidWhole(tid) && tidHasLock(tid, absLock); phase := collectorPhase; }
 
-yield procedure {:layer 95} ReadCollectorPhaseLocked({:layer 95} {:linear "tid"} tid: Tid) returns (phase:int)
+yield procedure {:layer 95} ReadCollectorPhaseLocked({:layer 95} {:linear} tid: Tid) returns (phase:int)
 refines AtomicReadCollectorPhaseLocked;
 {
     call phase := PrimitiveReadCollectorPhase();
 }
 
-both action {:layer 96} AtomicSetCollectorPhase({:linear "tid"} tid: Tid, phase:int)
+both action {:layer 96} AtomicSetCollectorPhase({:linear} tid: Tid, phase:int)
 modifies collectorPhase;
 { assert tid == GcTid && tidHasLock(tid, absLock); collectorPhase := phase; }
 
-yield procedure {:layer 95} SetCollectorPhase({:layer 95} {:linear "tid"} tid: Tid, phase:int)
+yield procedure {:layer 95} SetCollectorPhase({:layer 95} {:linear} tid: Tid, phase:int)
 refines AtomicSetCollectorPhase;
 {
     call PrimitiveSetCollectorPhase(phase);
 }
 
-both action {:layer 96,99} AtomicInitMutatorPhase({:linear "tid"} tid:Tid, {:linear "tid"} mutatorTids:[int]bool, id: int)
+both action {:layer 96,99} AtomicInitMutatorPhase({:linear} tid:Tid, {:linear} mutatorTids:Set Piece, id: int)
 modifies mutatorPhase;
 { assert gcAndMutatorTids(tid, mutatorTids); mutatorPhase[id] := IDLE(); }
 
-yield procedure {:layer 95} InitMutatorPhase({:layer 95} {:linear "tid"} tid:Tid, {:layer 95} {:linear "tid"} mutatorTids:[int]bool, id: int)
+yield procedure {:layer 95} InitMutatorPhase({:layer 95} {:linear} tid:Tid, {:layer 95} {:linear} mutatorTids:Set Piece, id: int)
 refines AtomicInitMutatorPhase;
 {
     call PrimitiveSetMutatorPhase(id, IDLE());
 }
 
-atomic action {:layer 96,100} AtomicReadMutatorPhaseByCollector({:linear "tid"} tid: Tid, i: int) returns (phase:int)
+atomic action {:layer 96,100} AtomicReadMutatorPhaseByCollector({:linear} tid: Tid, i: int) returns (phase:int)
 { assert tid == GcTid; phase := mutatorPhase[i]; }
 
-yield procedure {:layer 95} ReadMutatorPhaseByCollector({:layer 95} {:linear "tid"} tid: Tid, i: int) returns (phase:int)
+yield procedure {:layer 95} ReadMutatorPhaseByCollector({:layer 95} {:linear} tid: Tid, i: int) returns (phase:int)
 refines AtomicReadMutatorPhaseByCollector;
 {
     call phase := PrimitiveReadMutatorPhase(i);
 }
 
-both action {:layer 96,99} AtomicReadMutatorPhaseByMutator({:linear "tid"} tid: Tid, i: int) returns (phase:int)
+both action {:layer 96,99} AtomicReadMutatorPhaseByMutator({:linear} tid: Tid, i: int) returns (phase:int)
 { assert mutatorTidWhole(tid) && tid->i == i; phase := mutatorPhase[i]; }
 
-yield procedure {:layer 95} ReadMutatorPhaseByMutator({:layer 95} {:linear "tid"} tid: Tid, i: int) returns (phase:int)
+yield procedure {:layer 95} ReadMutatorPhaseByMutator({:layer 95} {:linear} tid: Tid, i: int) returns (phase:int)
 refines AtomicReadMutatorPhaseByMutator;
 {
     call phase := PrimitiveReadMutatorPhase(i);
 }
 
-atomic action {:layer 96} AtomicSetMutatorPhaseLocked({:linear "tid"} tid: Tid, i: int, phase: int)
+atomic action {:layer 96} AtomicSetMutatorPhaseLocked({:linear} tid: Tid, i: int, phase: int)
 modifies mutatorPhase;
 { assert mutatorTidWhole(tid) && tidHasLock(tid, absLock) && phase == collectorPhase && tid->i == i; mutatorPhase[i] := phase; }
 
-yield procedure {:layer 95} SetMutatorPhaseLocked({:layer 95} {:linear "tid"} tid: Tid, i: int, phase: int)
+yield procedure {:layer 95} SetMutatorPhaseLocked({:layer 95} {:linear} tid: Tid, i: int, phase: int)
 refines AtomicSetMutatorPhaseLocked;
 {
     call PrimitiveSetMutatorPhase(i, phase);
 }
 
-both action {:layer 96,99} AtomicInitSweepPtr({:linear "tid"} tid:Tid, {:linear "tid"} mutatorTids:[int]bool)
+both action {:layer 96,99} AtomicInitSweepPtr({:linear} tid:Tid, {:linear} mutatorTids:Set Piece)
 modifies sweepPtr;
 { assert gcAndMutatorTids(tid, mutatorTids); sweepPtr := memHi; }
 
-yield procedure {:layer 95} InitSweepPtr({:layer 95} {:linear "tid"} tid:Tid, {:layer 95} {:linear "tid"} mutatorTids:[int]bool)
+yield procedure {:layer 95} InitSweepPtr({:layer 95} {:linear} tid:Tid, {:layer 95} {:linear} mutatorTids:Set Piece)
 refines AtomicInitSweepPtr;
 {
     call PrimitiveSetSweepPtr(memHi);
 }
 
-both action {:layer 96} AtomicReadSweepPtr({:linear "tid"} tid:Tid) returns(val:int)
+both action {:layer 96} AtomicReadSweepPtr({:linear} tid:Tid) returns(val:int)
 { assert tidHasLock(tid, absLock); val := sweepPtr; }
 
-yield procedure {:layer 95} ReadSweepPtr({:layer 95} {:linear "tid"} tid:Tid) returns(val:int)
+yield procedure {:layer 95} ReadSweepPtr({:layer 95} {:linear} tid:Tid) returns(val:int)
 refines AtomicReadSweepPtr;
 {
     call val := PrimitiveReadSweepPtr();
 }
 
-atomic action {:layer 96} AtomicSetSweepPtrLocked({:linear "tid"} tid:Tid, val: int)
+atomic action {:layer 96} AtomicSetSweepPtrLocked({:linear} tid:Tid, val: int)
 modifies sweepPtr;
 { assert tid == GcTid && tidHasLock(tid, absLock); sweepPtr := val; }
 
-yield procedure {:layer 95} SetSweepPtrLocked({:layer 95} {:linear "tid"} tid:Tid, val: int)
+yield procedure {:layer 95} SetSweepPtrLocked({:layer 95} {:linear} tid:Tid, val: int)
 refines AtomicSetSweepPtrLocked;
 {
     call PrimitiveSetSweepPtr(val);
 }
 
-atomic action {:layer 96} AtomicCollectorRootScanBarrierStartLocked({:linear "tid"} tid: Tid)
+atomic action {:layer 96} AtomicCollectorRootScanBarrierStartLocked({:linear} tid: Tid)
 modifies rootScanOn;
 { assert tid == GcTid && tidHasLock(tid, absLock); rootScanOn := true; }
 
-yield procedure {:layer 95} CollectorRootScanBarrierStartLocked({:layer 95} {:linear "tid"} tid: Tid)
+yield procedure {:layer 95} CollectorRootScanBarrierStartLocked({:layer 95} {:linear} tid: Tid)
 refines AtomicCollectorRootScanBarrierStartLocked;
 {
     call PrimitiveSetRootScanOn(true);
 }
 
-atomic action {:layer 96} AtomicCollectorRootScanBarrierEndLocked({:linear "tid"} tid: Tid)
+atomic action {:layer 96} AtomicCollectorRootScanBarrierEndLocked({:linear} tid: Tid)
 modifies rootScanOn;
 { assert tid == GcTid && tidHasLock(tid, absLock); rootScanOn := false; }
 
-yield procedure {:layer 95} CollectorRootScanBarrierEndLocked({:layer 95} {:linear "tid"} tid: Tid)
+yield procedure {:layer 95} CollectorRootScanBarrierEndLocked({:layer 95} {:linear} tid: Tid)
 refines AtomicCollectorRootScanBarrierEndLocked;
 {
     call PrimitiveSetRootScanOn(false);
 }
 
-right action {:layer 96} AtomicMutatorReadBarrierOn({:linear "tid"} tid: Tid) returns (val:bool)
+right action {:layer 96} AtomicMutatorReadBarrierOn({:linear} tid: Tid) returns (val:bool)
 { assert tidHasLock(tid, absLock); val := rootScanOn; }
 
-yield procedure {:layer 95} MutatorReadBarrierOn({:layer 95} {:linear "tid"} tid: Tid) returns (val:bool)
+yield procedure {:layer 95} MutatorReadBarrierOn({:layer 95} {:linear} tid: Tid) returns (val:bool)
 refines AtomicMutatorReadBarrierOn;
 {
     call val := PrimitiveReadRootScanOn();
 }
 
-both action {:layer 96,99} AtomicPollMutatorReadBarrierOn({:linear "tid"} tid: Tid) returns (val:bool)
+both action {:layer 96,99} AtomicPollMutatorReadBarrierOn({:linear} tid: Tid) returns (val:bool)
 { }
 
-yield procedure {:layer 95} PollMutatorReadBarrierOn({:layer 95} {:linear "tid"} tid: Tid) returns (val:bool)
+yield procedure {:layer 95} PollMutatorReadBarrierOn({:layer 95} {:linear} tid: Tid) returns (val:bool)
 refines AtomicPollMutatorReadBarrierOn;
 {
     call val := PrimitiveReadRootScanOn();
 }
 
-atomic action {:layer 96,99} AtomicInitRootScanBarrier({:linear "tid"} tid:Tid, {:linear "tid"} mutatorTids:[int]bool)
+atomic action {:layer 96,99} AtomicInitRootScanBarrier({:linear} tid:Tid, {:linear} mutatorTids:Set Piece)
 modifies rootScanBarrier;
 { assert gcAndMutatorTids(tid, mutatorTids); rootScanBarrier := numMutators; }
 
-yield procedure {:layer 95} InitRootScanBarrier({:layer 95} {:linear "tid"} tid:Tid, {:layer 95} {:linear "tid"} mutatorTids:[int]bool)
+yield procedure {:layer 95} InitRootScanBarrier({:layer 95} {:linear} tid:Tid, {:layer 95} {:linear} mutatorTids:Set Piece)
 refines AtomicInitRootScanBarrier;
 {
     call PrimitiveSetRootScanBarrier(numMutators);
 }
 
-atomic action {:layer 96} AtomicCollectorRootScanBarrierRead({:linear "tid"} tid: Tid) returns (val:int)
+atomic action {:layer 96} AtomicCollectorRootScanBarrierRead({:linear} tid: Tid) returns (val:int)
 { assert tid == GcTid; val := rootScanBarrier; }
 
-yield procedure {:layer 95} CollectorRootScanBarrierRead({:layer 95} {:linear "tid"} tid: Tid) returns (val:int)
+yield procedure {:layer 95} CollectorRootScanBarrierRead({:layer 95} {:linear} tid: Tid) returns (val:int)
 refines AtomicCollectorRootScanBarrierRead;
 {
     call val := PrimitiveReadRootScanBarrier();
 }
 
-atomic action {:layer 96} AtomicAddRootScanBarrier({:linear "tid"} tid_left: Tid, val: int)
+atomic action {:layer 96} AtomicAddRootScanBarrier({:linear} tid_left: Tid, val: int)
 modifies rootScanBarrier;
 { assert mutatorTidLeft(tid_left) && tidHasLock(tid_left, absLock); rootScanBarrier := rootScanBarrier + val; }
 
-yield procedure {:layer 95} AddRootScanBarrier({:layer 95} {:linear "tid"} tid_left: Tid, val: int)
+yield procedure {:layer 95} AddRootScanBarrier({:layer 95} {:linear} tid_left: Tid, val: int)
 refines AtomicAddRootScanBarrier;
 {
     call PrimitiveAddRootScanBarrier(val);
 }
 
-right action {:layer 96} AtomicMutatorsInRootScanBarrierAdd({:linear "tid"} tid_left: Tid, {:linear_in "tid"} tid_right: Tid)
+right action {:layer 96} AtomicMutatorsInRootScanBarrierAdd({:linear} tid_left: Tid, {:linear_in} tid_right: Tid)
 modifies mutatorsInRootScanBarrier;
 {
+    var i: int;
+    var {:linear} ps: Set Piece;
+    var {:linear} p: One Piece;
     assert tidHasLock(tid_left, absLock) && mutatorTidRight(tid_right);
-    mutatorsInRootScanBarrier[tid_right->i] := true;
+    Tid(i, ps) := tid_right;
+    call p := One_Get(ps, Right(i));
+    call One_Put(mutatorsInRootScanBarrier, p);
 }
 
-yield procedure {:layer 95} MutatorsInRootScanBarrierAdd({:layer 95} {:linear "tid"} tid_left: Tid, {:layer 95} {:linear_in "tid"} tid_right: Tid)
+yield procedure {:layer 95} MutatorsInRootScanBarrierAdd({:layer 95} {:linear} tid_left: Tid, {:layer 95} {:linear_in} tid_right: Tid)
 refines AtomicMutatorsInRootScanBarrierAdd;
 {
     call {:layer 95} mutatorsInRootScanBarrier := PrimitiveMutatorsInRootScanBarrierAdd(tid_right, mutatorsInRootScanBarrier);
 }
 
-both action {:layer 96} AtomicMutatorsInRootScanBarrierRemove({:linear "tid"} tid_left: Tid) returns({:linear "tid"} tid_right: Tid)
+both action {:layer 96} AtomicMutatorsInRootScanBarrierRemove({:linear} tid_left: Tid) returns({:linear} tid_right: Tid)
 modifies mutatorsInRootScanBarrier;
 {
-    assert tidHasLock(tid_left, absLock) && !rootScanOn && mutatorTidLeft(tid_left) && mutatorsInRootScanBarrier[tid_left->i];
-    mutatorsInRootScanBarrier[tid_left->i] := false;
-    tid_right := Tid(tid_left->i, false, true);
+    var {:linear} ps: Set Piece;
+    assert tidHasLock(tid_left, absLock) && !rootScanOn && mutatorTidLeft(tid_left) && Set_Contains(mutatorsInRootScanBarrier, Right(tid_left->i));
+    call ps := Set_Get(mutatorsInRootScanBarrier, MapOne(Right(tid_left->i)));
+    tid_right := Tid(tid_left->i, ps);
 }
 
-yield procedure {:layer 95} MutatorsInRootScanBarrierRemove({:layer 95} {:linear "tid"} tid_left: Tid) returns({:layer 95} {:linear "tid"} tid_right: Tid)
+yield procedure {:layer 95} MutatorsInRootScanBarrierRemove({:layer 95} {:linear} tid_left: Tid) returns({:layer 95} {:linear} tid_right: Tid)
 refines AtomicMutatorsInRootScanBarrierRemove;
 ensures {:layer 95} tid_left->i == tid_right->i;
-ensures {:layer 95} tid_left->left && tid_right->right;
+ensures {:layer 95} Set_Contains(tid_left->ps, Left(tid_left->i)) && Set_Contains(tid_right->ps, Right(tid_right->i));
 {
     call {:layer 95} tid_right, mutatorsInRootScanBarrier := PrimitiveMutatorsInRootScanBarrierRemove(tid_left, mutatorsInRootScanBarrier);
 }
 
-both action {:layer 96,99} AtomicInitRoot({:linear "tid"} tid:Tid, {:linear "tid"} mutatorTids:[int]bool, x: int)
+both action {:layer 96,99} AtomicInitRoot({:linear} tid:Tid, {:linear} mutatorTids:Set Piece, x: int)
 modifies root;
 { assert gcAndMutatorTids(tid, mutatorTids) && rootAddr(x); root[x] := 0; }
 
-yield procedure {:layer 95} InitRoot({:layer 95} {:linear "tid"} tid:Tid, {:layer 95} {:linear "tid"} mutatorTids:[int]bool, x: int)
+yield procedure {:layer 95} InitRoot({:layer 95} {:linear} tid:Tid, {:layer 95} {:linear} mutatorTids:Set Piece, x: int)
 refines AtomicInitRoot;
 {
     call PrimitiveWriteRoot(x, 0);
 }
 
-left action {:layer 96,99} AtomicReadRootInRootScanBarrier({:linear "tid"} tid:Tid, x: idx) returns (val: int)
+left action {:layer 96,99} AtomicReadRootInRootScanBarrier({:linear} tid:Tid, x: idx) returns (val: int)
 { assert tid == GcTid && rootAddr(x) && rootScanOn && mutatorsInRootScanBarrier == Mutators; val := root[x]; }
 
-yield procedure {:layer 95} ReadRootInRootScanBarrier({:layer 95} {:linear "tid"} tid:Tid, x: idx) returns (val: int)
+yield procedure {:layer 95} ReadRootInRootScanBarrier({:layer 95} {:linear} tid:Tid, x: idx) returns (val: int)
 refines AtomicReadRootInRootScanBarrier;
 {
     call val := PrimitiveReadRoot(x);
 }
 
-both action {:layer 96,99} AtomicWriteRoot({:linear "tid"} tid: Tid, i: idx, val: int)
+both action {:layer 96,99} AtomicWriteRoot({:linear} tid: Tid, i: idx, val: int)
 modifies root;
 { assert mutatorTidWhole(tid) && rootAddr(i) && tidOwns(tid, i); root[i] := val; }
 
-yield procedure {:layer 95} WriteRoot({:layer 95} {:linear "tid"} tid: Tid, i: idx, val: int)
+yield procedure {:layer 95} WriteRoot({:layer 95} {:linear} tid: Tid, i: idx, val: int)
 refines AtomicWriteRoot;
 {
     call PrimitiveWriteRoot(i, val);
 }
 
-both action {:layer 96,99} AtomicReadRoot({:linear "tid"} tid: Tid, i: idx) returns (val: int)
+both action {:layer 96,99} AtomicReadRoot({:linear} tid: Tid, i: idx) returns (val: int)
 { assert mutatorTidWhole(tid) && rootAddr(i) && tidOwns(tid, i); val := root[i]; }
 
-yield procedure {:layer 95} ReadRoot({:layer 95} {:linear "tid"} tid: Tid, i: idx) returns (val: int)
+yield procedure {:layer 95} ReadRoot({:layer 95} {:linear} tid: Tid, i: idx) returns (val: int)
 refines AtomicReadRoot;
 {
     call val := PrimitiveReadRoot(i);
 }
 
-both action {:layer 96,99} AtomicInitColor({:linear "tid"} tid:Tid, {:linear "tid"} mutatorTids:[int]bool, x: int)
+both action {:layer 96,99} AtomicInitColor({:linear} tid:Tid, {:linear} mutatorTids:Set Piece, x: int)
 modifies Color;
 { assert gcAndMutatorTids(tid, mutatorTids) && memAddr(x); Color[x] := UNALLOC(); }
 
-yield procedure {:layer 95} InitColor({:layer 95} {:linear "tid"} tid:Tid, {:layer 95} {:linear "tid"} mutatorTids:[int]bool, x: int)
+yield procedure {:layer 95} InitColor({:layer 95} {:linear} tid:Tid, {:layer 95} {:linear} mutatorTids:Set Piece, x: int)
 refines AtomicInitColor;
 {
     call PrimitiveSetColor(x, UNALLOC());
 }
 
-both action {:layer 96} AtomicReadColorByCollector({:linear "tid"} tid:Tid, i: int) returns (val: int)
+both action {:layer 96} AtomicReadColorByCollector({:linear} tid:Tid, i: int) returns (val: int)
 { assert tid == GcTid && tidHasLock(tid, absLock) && memAddr(i); val := Color[i]; }
 
-yield procedure {:layer 95} ReadColorByCollector({:layer 95} {:linear "tid"} tid:Tid, i: int) returns (val: int)
+yield procedure {:layer 95} ReadColorByCollector({:layer 95} {:linear} tid:Tid, i: int) returns (val: int)
 refines AtomicReadColorByCollector;
 {
     call val := PrimitiveReadColor(i);
 }
 
-atomic action {:layer 96} AtomicReadColorByMutator1({:linear "tid"} tid:Tid, i: int) returns (val: int)
+atomic action {:layer 96} AtomicReadColorByMutator1({:linear} tid:Tid, i: int) returns (val: int)
 { assert mutatorTidWhole(tid) && memAddr(i); }
 
-yield procedure {:layer 95} ReadColorByMutator1({:layer 95} {:linear "tid"} tid:Tid, i: int) returns (val: int)
+yield procedure {:layer 95} ReadColorByMutator1({:layer 95} {:linear} tid:Tid, i: int) returns (val: int)
 refines AtomicReadColorByMutator1;
 {
     call val := PrimitiveReadColor(i);
 }
 
-both action {:layer 96} AtomicReadColorByMutator2({:linear "tid"} tid:Tid, i: int) returns (val: int)
+both action {:layer 96} AtomicReadColorByMutator2({:linear} tid:Tid, i: int) returns (val: int)
 { assert mutatorTidWhole(tid) && tidHasLock(tid, absLock) && memAddr(i); val := Color[i]; }
 
-yield procedure {:layer 95} ReadColorByMutator2({:layer 95} {:linear "tid"} tid:Tid, i: int) returns (val: int)
+yield procedure {:layer 95} ReadColorByMutator2({:layer 95} {:linear} tid:Tid, i: int) returns (val: int)
 refines AtomicReadColorByMutator2;
 {
     call val := PrimitiveReadColor(i);
 }
 
-atomic action {:layer 96,98} AtomicReadColorByMutator3({:linear "tid"} tid:Tid, i: int) returns (val: int)
+atomic action {:layer 96,98} AtomicReadColorByMutator3({:linear} tid:Tid, i: int) returns (val: int)
 {
     assert mutatorTidWhole(tid) && memAddr(i) && MarkPhase(mutatorPhase[tid->i]);
     assume White(Color[i]) ==> White(val);
 }
 
-yield procedure {:layer 95} ReadColorByMutator3({:layer 95} {:linear "tid"} tid:Tid, i: int) returns (val: int)
+yield procedure {:layer 95} ReadColorByMutator3({:layer 95} {:linear} tid:Tid, i: int) returns (val: int)
 refines AtomicReadColorByMutator3;
 {
     call val := PrimitiveReadColor(i);
 }
 
-both action {:layer 96} AtomicSetColor({:linear "tid"} tid:Tid, i: int, val: int)
+both action {:layer 96} AtomicSetColor({:linear} tid:Tid, i: int, val: int)
 modifies Color;
 { assert tidHasLock(tid, absLock) && memAddr(i) && PhaseConsistent(collectorPhase, mutatorPhase) && !MarkPhase(collectorPhase); Color[i] := val; }
 
-yield procedure {:layer 95} SetColor({:layer 95} {:linear "tid"} tid:Tid, i: int, val: int)
+yield procedure {:layer 95} SetColor({:layer 95} {:linear} tid:Tid, i: int, val: int)
 refines AtomicSetColor;
 {
     call PrimitiveSetColor(i, val);
 }
 
-left action {:layer 96} AtomicSetColorInMarkPhase({:linear "tid"} tid:Tid, i: int, val: int)
+left action {:layer 96} AtomicSetColorInMarkPhase({:linear} tid:Tid, i: int, val: int)
 modifies Color;
 {
     assert tidHasLock(tid, absLock) && memAddr(i);
@@ -1884,13 +1885,13 @@ modifies Color;
     Color[i] := val;
 }
 
-yield procedure {:layer 95} SetColorInMarkPhase({:layer 95} {:linear "tid"} tid:Tid, i: int, val: int)
+yield procedure {:layer 95} SetColorInMarkPhase({:layer 95} {:linear} tid:Tid, i: int, val: int)
 refines AtomicSetColorInMarkPhase;
 {
     call PrimitiveSetColor(i, val);
 }
 
-atomic action {:layer 96} AtomicSetColorInAlloc({:linear "tid"} tid:Tid, i: int, val: int, o: obj)
+atomic action {:layer 96} AtomicSetColorInAlloc({:linear} tid:Tid, i: int, val: int, o: obj)
 modifies Color, toAbs;
 {
     assert tidHasLock(tid, absLock) && memAddr(i);
@@ -1899,31 +1900,31 @@ modifies Color, toAbs;
     toAbs[i] := o;
 }
 
-yield procedure {:layer 95} SetColorInAlloc({:layer 95} {:layer 95} {:linear "tid"} tid:Tid, i: int, val: int, o: obj)
+yield procedure {:layer 95} SetColorInAlloc({:layer 95} {:layer 95} {:linear} tid:Tid, i: int, val: int, o: obj)
 refines AtomicSetColorInAlloc;
 {
     call PrimitiveSetColor(i, val);
     call {:layer 95} toAbs := Copy(toAbs[i := o]);
 }
 
-both action {:layer 96,99} AtomicInitToAbs({:linear "tid"} tid:Tid, {:linear "tid"} mutatorTids:[int]bool)
+both action {:layer 96,99} AtomicInitToAbs({:linear} tid:Tid, {:linear} mutatorTids:Set Piece)
 modifies toAbs;
 {
     assert gcAndMutatorTids(tid, mutatorTids);
     toAbs := (lambda i:int :: if memAddr(i) then nil else Int(i));
 }
 
-yield procedure {:layer 95} InitToAbs({:layer 95} {:linear "tid"} tid:Tid, {:layer 95} {:linear "tid"} mutatorTids:[int]bool)
+yield procedure {:layer 95} InitToAbs({:layer 95} {:linear} tid:Tid, {:layer 95} {:linear} mutatorTids:Set Piece)
 refines AtomicInitToAbs;
 {
     call {:layer 95} toAbs := Copy((lambda i:int :: if memAddr(i) then nil else Int(i)));
 }
 
-right action {:layer 96} AtomicLockAcquire({:linear "tid"} tid: Tid)
+right action {:layer 96} AtomicLockAcquire({:linear} tid: Tid)
 modifies absLock;
 { assert tid->i != 0; assume absLock == 0; absLock := tid->i; }
 
-yield procedure {:layer 95} LockAcquire({:layer 95} {:linear "tid"} tid: Tid)
+yield procedure {:layer 95} LockAcquire({:layer 95} {:linear} tid: Tid)
 refines AtomicLockAcquire;
 preserves call Yield_Lock();
 {
@@ -1941,11 +1942,11 @@ preserves call Yield_Lock();
     }
 }
 
-left action {:layer 96} AtomicLockRelease({:linear "tid"} tid:Tid)
+left action {:layer 96} AtomicLockRelease({:linear} tid:Tid)
 modifies absLock;
 { assert tidHasLock(tid, absLock); absLock := 0; }
 
-yield procedure {:layer 95} LockRelease({:layer 95} {:linear "tid"} tid:Tid)
+yield procedure {:layer 95} LockRelease({:layer 95} {:linear} tid:Tid)
 refines AtomicLockRelease;
 preserves call Yield_Lock();
 {
@@ -1962,14 +1963,28 @@ invariant lock <==> absLock != 0;
 //   (Note, though, that Boogie still verifies the mover types (atomic,left,right,both); these are not trusted.)
 //////////////////////////////////////////////////////////////////////////////
 
-pure action TidSplit({:linear_in "tid"} tid:Tid) returns({:linear "tid"} tid_left:Tid, {:linear "tid"} tid_right:Tid)
-{ assert tid->left && tid->right; tid_left := Tid(tid->i, true, false); tid_right := Tid(tid->i, false, true); }
+pure action TidSplit({:linear_in} tid:Tid) returns({:linear} tid_left:Tid, {:linear} tid_right:Tid)
+{
+    var i: int;
+    var {:linear} ps_right: Set Piece;
+    i := tid->i;
+    tid_left := tid;
+    ps_right := Set_Singleton(Right(i));
+    call Set_Split(tid_left->ps, ps_right);
+    tid_right := Tid(i, ps_right);
+}
 
-pure action TidCombine({:linear_in "tid"} tid_left:Tid, {:linear_in "tid"} tid_right:Tid) returns({:linear "tid"} tid:Tid)
-{ assert tid_left->i == tid_right->i && tid_left->left && tid_right->right; tid := Tid(tid_left->i, true, true); }
-
-pure action TidOutput({:linear_in "tid"} tid_in:Tid, {:linear_out "tid"} tid_out:Tid)
-{ assert tid_in == tid_out; }
+pure action TidCombine({:linear_in} tid_left:Tid, {:linear_in} tid_right:Tid) returns({:linear} tid:Tid)
+{
+    var i: int;
+    var {:linear} ps_right: Set Piece;
+    var {:linear} p: One Piece;
+    assert tid_left->i == tid_right->i;
+    tid := tid_left;
+    Tid(i, ps_right) := tid_right;
+    call p := One_Get(ps_right, Right(i));
+    call One_Put(tid->ps, p);
+}
 
 atomic action {:layer 1,95} AtomicPrimitiveReadField(x: int, f: fld) returns (y: int)
 { assert memAddr(x) && fieldAddr(f); y := mem[x][f]; }
@@ -2065,19 +2080,27 @@ modifies rootScanBarrier;
 yield procedure {:layer 0} PrimitiveAddRootScanBarrier(val: int);
 refines AtomicPrimitiveAddRootScanBarrier;
 
-pure action PrimitiveMutatorsInRootScanBarrierAdd({:linear_in "tid"} tid_right: Tid, {:linear_in "tid"} mutatorsInRootScanBarrier: [int]bool)
-    returns ({:linear "tid"} mutatorsInRootScanBarrier': [int]bool)
+pure action PrimitiveMutatorsInRootScanBarrierAdd({:linear_in} tid_right: Tid, {:linear_in} mutatorsInRootScanBarrier: Set Piece)
+    returns ({:linear} mutatorsInRootScanBarrier': Set Piece)
 {
+    var i: int;
+    var {:linear} ps: Set Piece;
+    var {:linear} p: One Piece;
     assert mutatorTidRight(tid_right);
-    mutatorsInRootScanBarrier' := mutatorsInRootScanBarrier[tid_right->i := true];
+    Tid(i, ps) := tid_right;
+    call p := One_Get(ps, Right(i));
+    mutatorsInRootScanBarrier' := mutatorsInRootScanBarrier;
+    call One_Put(mutatorsInRootScanBarrier', p);
 }
 
-pure action PrimitiveMutatorsInRootScanBarrierRemove({:linear "tid"} tid_left: Tid, {:linear_in "tid"} mutatorsInRootScanBarrier: [int]bool)
-    returns({:linear "tid"} tid_right: Tid, {:linear "tid"} mutatorsInRootScanBarrier': [int]bool)
+pure action PrimitiveMutatorsInRootScanBarrierRemove({:linear} tid_left: Tid, {:linear_in} mutatorsInRootScanBarrier: Set Piece)
+    returns({:linear} tid_right: Tid, {:linear} mutatorsInRootScanBarrier': Set Piece)
 {
-    assert mutatorTidLeft(tid_left) && mutatorsInRootScanBarrier[tid_left->i];
-    mutatorsInRootScanBarrier' := mutatorsInRootScanBarrier[tid_left->i := false];
-    tid_right := Tid(tid_left->i, false, true);
+    var {:linear} ps: Set Piece;
+    assert mutatorTidLeft(tid_left);
+    mutatorsInRootScanBarrier' := mutatorsInRootScanBarrier;
+    call ps := Set_Get(mutatorsInRootScanBarrier', MapOne(Right(tid_left->i)));
+    tid_right := Tid(tid_left->i, ps);
 }
 
 atomic action {:layer 1,95} AtomicPrimitiveWriteRoot(i: idx, val: int)
